Charge!/src/Charge/ModularFunc/BaseFunc.v
@@ -1,0 +1,194 @@
+Require Import ExtLib.Core.RelDec.
+Require Import ExtLib.Data.Fun.
+Require Import ExtLib.Data.Nat.
+Require Import ExtLib.Data.Bool.
+Require Import ExtLib.Data.String.
+Require Import ExtLib.Tactics.Consider.
+
+Require Import MirrorCore.TypesI.
+Require Import MirrorCore.syms.SymEnv.
+Require Import MirrorCore.Lambda.Expr.
+
+Require Import Charge.Logics.ILogic.
+Require Import Charge.ModularFunc.BaseType.
+
+Require Import Coq.Strings.String.
+
+
+Set Implicit Arguments.
+Set Strict Implicit.
+Set Maximal Implicit Insertion.
+
+Inductive base_func typ :=
+  | pNat : nat -> base_func typ
+  | pBool : bool -> base_func typ
+  | pString : string -> base_func typ
+  | pEq : typ -> base_func typ
+  | pPair : typ -> typ -> base_func typ.
+
+Class BaseFunc (typ func : Type) := {
+  fNat  : nat -> func;
+  fBool : bool -> func;
+  fString : string -> func;
+  
+  fEq : typ -> func;
+  fPair : typ -> typ -> func;
+  
+  baseS : func -> option (base_func typ)
+}.
+
+    
+Section BaseFuncSum.
+	Context {typ func : Type} {H : BaseFunc typ func}.
+
+	Global Instance BaseFuncSumL (A : Type) : 
+		BaseFunc typ (func + A) := {
+		  fNat n := inl (fNat n)
+	    ; fBool b := inl (fBool b)
+	    ; fString s := inl (fString s)
+        ; fEq t := inl (fEq t)
+        ; fPair t1 t2 := inl (fPair t1 t2)
+        ; baseS f := match f with
+        			   | inl a => baseS a
+        			   | inr _ => None
+        			 end
+        }.
+
+	Global Instance BaseFuncSumR (A : Type) : 
+		BaseFunc typ (A + func) := {
+		  fNat n := inr (fNat n)
+	    ; fBool b := inr (fBool b)
+	    ; fString s := inr (fString s)
+        ; fEq t := inr (fEq t)
+        ; fPair t1 t2 := inr (fPair t1 t2)
+        ; baseS f := match f with
+        			   | inr a => baseS a
+        			   | inl _ => None
+        			 end
+        }.
+        
+    Global Instance BaseFuncExpr :
+    	BaseFunc typ (expr typ func) := {
+    	  fNat n := Inj (fNat n);
+    	  fBool b := Inj (fBool b);
+    	  fString s := Inj (fString s);
+    	  fEq t := Inj (fEq t);
+    	  fPair t1 t2 := Inj (fPair t1 t2);
+    	  baseS f := match f with
+    	  			   | Inj f => baseS f
+    	  			   | _     => None
+    	  			 end
+    }.
+
+End BaseFuncSum.
+
+Section BaseFuncInst.
+	Context {typ : Type} {HR : RType typ} 
+	        {HT : BaseType typ} {HTD: BaseTypeD}.
+	Context {func : Type} {H : BaseFunc typ func}.
+	Context {Heq : RelDec (@eq typ)} {HC : RelDec_Correct Heq}.
+
+    Variable Typ2_tyArr : Typ2 _ Fun.
+    Variable Typ0_tyProp : Typ0 _ Prop.
+
+    Let tyArr : typ -> typ -> typ := @typ2 _ _ _ _.
+    Let tyProp : typ := @typ0 _ _ _ _.
+
+	Global Instance BaseFuncInst : BaseFunc typ (base_func typ) := {
+	  fNat := pNat typ;
+	  fBool := pBool typ;
+	  fString := pString typ;
+	  fEq := pEq;
+	  fPair := pPair;
+	  baseS f := Some f 
+	}.
+
+	Definition typeof_base_func bf :=
+		match bf with
+		  | pNat _ => Some tyNat
+		  | pBool _ => Some tyBool
+		  | pString _ => Some tyString
+		  | pEq t => Some (tyArr t (tyArr t tyProp))
+		  | pPair t1 t2 => Some (tyArr t1 (tyArr t2 (tyPair t1 t2)))
+		end.
+
+	Definition base_func_eq (a b : base_func typ) : option bool :=
+	  match a , b with
+	    | pNat a, pNat b => Some (a ?[ eq ] b)
+	    | pBool a, pBool b => Some (a ?[ eq ] b)
+	    | pString a, pString b => Some (a ?[ eq ] b)
+	    | pEq t1, pEq t2 => Some (t1 ?[ eq ] t2)
+	    | pPair t1 t2, pPair t3 t4 => Some (t1 ?[ eq ] t3 &&
+	      								    t2 ?[ eq ] t4)%bool
+	    | _, _ => None
+	  end.
+
+    Global Instance RelDec_base_func : RelDec (@eq (base_func typ)) := {
+      rel_dec a b := match base_func_eq a b with 
+    	  		       | Some b => b 
+    		 	       | None => false 
+    			     end
+    }.
+
+    Global Instance RelDec_Correct_ilfunc : RelDec_Correct RelDec_base_func.
+    Proof.
+      constructor.
+      destruct x; destruct y; simpl;
+      try solve [ try rewrite Bool.andb_true_iff ;
+                  repeat rewrite rel_dec_correct; intuition congruence ].
+    Qed.
+  
+	 Definition base_func_symD bf :=
+		match bf as bf return match typeof_base_func bf with
+								| Some t => typD t
+								| None => unit
+							  end with
+	    | pNat n => eq_rect_r id n btNat
+	    | pBool b => eq_rect_r id b btBool
+	    | pString s => eq_rect_r id s btString
+	    | pEq t => 
+	       eq_rect_r id
+             (eq_rect_r (fun T : Type => typD t -> T)
+               (fun A B : typD t => eq_rect_r id (A = B)
+                                    (typ0_cast (F:=Prop)))
+               (typ2_cast t tyProp))
+             (typ2_cast t (typ2 t tyProp))
+        | pPair t1 t2 => 
+           eq_rect_r id 
+             (eq_rect_r (fun T : Type => typD t1 -> T)
+               (fun (A : typD t1) (B : typD t2) => 
+               	     eq_rect_r id (A, B) (btPair t1 t2))
+               (typ2_cast t2 (tyPair t1 t2)))
+             (typ2_cast t1 (typ2 t2 (tyPair t1 t2)))
+	end.
+
+	Global Instance RSym_BaseFunc : SymI.RSym (base_func typ) := {
+	  typeof_sym := typeof_base_func;
+	  symD := base_func_symD;
+	  sym_eqb := base_func_eq
+	}.
+
+	Global Instance RSymOk_BaseFunc : SymI.RSymOk RSym_BaseFunc.
+	Proof.
+		split; intros.
+		destruct a, b; simpl; try apply I.
+		+ consider (n ?[ eq ] n0); intuition congruence.
+		+ consider (b0 ?[ eq ] b); intuition congruence.
+		+ consider (s ?[ eq ] s0); intuition congruence.
+		+ consider (t ?[ eq ] t0); intuition congruence.
+		+ consider (t ?[ eq ] t1 && t0 ?[ eq ] t2)%bool; 
+		  intuition congruence.
+	Qed.
+
+End BaseFuncInst.
+
+Section MakeBase.
+	Context {typ func : Type} {H : BaseFunc typ func}.
+
+	Definition mkNat n : expr typ func := Inj (fNat n).
+	Definition mkBool b : expr typ func := Inj (fBool b).
+	Definition mkString s : expr typ func := Inj (fString s).
+	Definition mkEq (t : typ) (a b : expr typ func) := App (App (fEq t) a) b.
+	Definition mkPair t u a b := App (App (fPair t u) a) b.
+
+End MakeBase.
