Charge!/src/Charge/ModularFunc/EmbedFunc.v
@@ -1,0 +1,184 @@
+Require Import ExtLib.Core.RelDec.
+Require Import ExtLib.Data.Fun.
+Require Import ExtLib.Data.Nat.
+Require Import ExtLib.Data.Bool.
+Require Import ExtLib.Data.String.
+Require Import ExtLib.Tactics.Consider.
+
+Require Import MirrorCore.TypesI.
+Require Import MirrorCore.syms.SymEnv.
+Require Import MirrorCore.Lambda.Expr.
+Require Import MirrorCore.SymI.
+
+Require Import Charge.Logics.ILogic.
+Require Import Charge.Logics.ILEmbed.
+Require Import Charge.ModularFunc.ILogicFunc.
+
+Require Import Coq.Strings.String.
+Require Import Coq.Bool.Bool.
+
+
+Set Implicit Arguments.
+Set Strict Implicit.
+Set Maximal Implicit Insertion.
+
+Inductive embed_func typ :=
+  | eilf_embed (_ _ : typ).
+    
+Class EmbedFunc (typ func : Type) := {
+  fEmbed : typ -> typ -> func;
+  embedS : func -> option (embed_func typ)
+}.
+    
+Section EmbedFuncSum.
+	Context {typ func : Type} {H : EmbedFunc typ func}.
+
+	Global Instance EmbedFuncSumL (A : Type) : 
+	   EmbedFunc typ (func + A) := {
+		  fEmbed t u := inl (fEmbed t u);
+		  embedS f := match f with
+		  				| inl f => embedS f
+		  				| inr _ => None
+		  			  end
+       }.
+
+	Global Instance EmbedFuncSumR (A : Type) : 
+		EmbedFunc typ (A + func) := {
+		  fEmbed t u := inr (fEmbed t u);
+		  embedS f := match f with
+		  				| inr f => embedS f
+		  				| inl _ => None
+		  			  end
+       }.
+
+	Global Instance EmbedFuncExpr : 
+		EmbedFunc typ (expr typ func) := {
+		  fEmbed t u := Inj (fEmbed t u);
+		  embedS f := match f with
+		  				| Inj f => embedS f
+		  				| _ => None
+		  			  end
+        }.
+
+End EmbedFuncSum.
+
+Section EmbedFuncInst.
+
+	Context {typ func : Type} {H : EmbedFunc typ func}.
+	Context {HR : RType typ} {Heq : RelDec (@eq typ)} {HC : RelDec_Correct Heq}.
+
+    Variable Typ2_tyArr : Typ2 _ Fun.
+    Variable Typ0_tyProp : Typ0 _ Prop.
+
+    Let tyArr : typ -> typ -> typ := @typ2 _ _ _ _.
+    Let tyProp : typ := @typ0 _ _ _ _.
+
+	Global Instance EmbedFuncInst : EmbedFunc typ (embed_func typ) := {
+	  fEmbed := eilf_embed;
+	  embedS f := Some f
+	}.
+	
+  Variable is : logic_ops.
+
+ 
+  Definition embed_ops := forall (t u : typ),
+    option (EmbedOp (typD t) (typD u)).
+  Definition embed_opsOk (es : embed_ops) : Prop :=
+    forall t t',
+      match is t , is t' , es t t' return Prop with
+        | Some a , Some b , Some T => @Embed _ a _ _ T
+        | _ , _ , _ => True
+      end.
+
+  Variable gs : embed_ops.
+  
+  Definition typeof_embed_func (f : embed_func typ) : option typ :=
+    match f with
+      | eilf_embed t u => match gs t u with
+				  	        | Some _ => Some (tyArr t u)
+				  	        | None => None
+				  	      end
+  	end.
+
+  Global Instance RelDec_embed_func : RelDec (@eq (embed_func typ)) :=
+  { rel_dec := fun a b =>
+	         match a, b with
+	  	       | eilf_embed t u, eilf_embed t' u' => (t ?[eq] t' && u ?[ eq ] u')%bool
+	         end
+  }.
+
+  Global Instance RelDec_Correct_embed_func : RelDec_Correct RelDec_embed_func.
+  Proof.
+    constructor.
+    destruct x; destruct y; simpl; rewrite andb_true_iff;
+    repeat rewrite rel_dec_correct; intuition congruence.
+  Qed.
+  
+  Definition typ2_cast' (a b : typ)
+  	: (typD a -> typD b) -> typD (tyArr a b) := 
+  		fun f =>
+  		match eq_sym (typ2_cast a b) in _ = t return t with
+  			| eq_refl => f
+  		end.
+
+  Definition typ2_cast_bin (a b c : typ)
+  : (typD a -> typD b -> typD c) -> typD (tyArr a (tyArr b c)) :=
+    fun f =>
+      match eq_sym (typ2_cast a (tyArr b c)) in _ = t
+            return t with
+        | eq_refl => match eq_sym (typ2_cast b c) in _ = t
+                           return _ -> t with
+                       | eq_refl => f
+                     end
+        end.
+
+ Definition funcD (f : embed_func typ) : match typeof_embed_func f with
+							              | Some t => typD t
+							              | None => unit
+							             end :=
+    match f as f
+          return match typeof_embed_func f with
+		   | Some t => typD t
+		   | None => unit
+		 end
+    with
+      | eilf_embed t u =>
+        match gs t u as x
+              return match match x with
+			     | Some _ => Some (tyArr t u)
+			     | None => None
+			   end with
+		       | Some t0 => typD t0
+		       | None => unit
+		     end
+        with
+	  | Some t0 =>
+            match eq_sym (typ2_cast t u) in _ = t return t
+            with
+              | eq_refl => @embed _ _ _
+            end
+	  | None => tt
+        end
+    end.
+
+  Global Instance RSym_embed_func : SymI.RSym (embed_func typ) :=
+  { typeof_sym := typeof_embed_func
+  ; sym_eqb := fun a b => Some (rel_dec a b)
+  ; symD := funcD
+  }.
+
+  Global Instance RSymOk_embed_func : SymI.RSymOk RSym_embed_func.
+  Proof.
+    constructor.
+    intros. unfold sym_eqb; simpl.
+    consider (a ?[ eq ] b); auto.
+  Qed.
+
+End EmbedFuncInst.
+
+Section MakeEmbed.
+	Context {typ func : Type} {H : EmbedFunc typ func}.
+
+	Definition mkEmbed (t u : typ) P := App (fEmbed t u) P.
+
+End MakeEmbed.
