Charge!/src/Charge/ModularFunc/ILogicFunc.v
@@ -1,0 +1,693 @@
+Require Import ExtLib.Core.RelDec.
+Require Import ExtLib.Data.Fun.
+Require Import ExtLib.Data.Nat.
+Require Import ExtLib.Data.Bool.
+Require Import ExtLib.Data.String.
+Require Import ExtLib.Tactics.
+Require Import ExtLib.Tactics.Consider.
+
+Require Import MirrorCore.TypesI.
+Require Import MirrorCore.syms.SymEnv.
+Require Import MirrorCore.Lambda.Expr.
+Require Import MirrorCore.SymI.
+Require Import MirrorCore.syms.SymSum.
+
+Require Import Charge.Logics.ILogic.
+
+Require Import Coq.Strings.String.
+Require Import Coq.Bool.Bool.
+
+Set Implicit Arguments.
+Set Strict Implicit.
+Set Maximal Implicit Insertion.
+
+Inductive ilfunc typ :=
+  | ilf_entails (logic : typ)
+  | ilf_true (logic : typ)
+  | ilf_false (logic : typ)
+  | ilf_and (logic : typ)
+  | ilf_or (logic : typ)
+  | ilf_impl (logic : typ)
+  | ilf_exists (arg logic : typ)
+  | ilf_forall (arg logic : typ).
+  
+Definition ilfunc_logic typ (x : ilfunc typ) : typ :=
+  match x with
+    | ilf_entails t => t
+    | ilf_true t => t
+    | ilf_false t => t
+    | ilf_and t => t
+    | ilf_or t => t
+    | ilf_impl t => t
+    | ilf_exists _ t => t
+    | ilf_forall _ t => t
+  end.
+
+Class ILogicFunc (typ func : Type) := {
+  fEntails  : typ -> func;
+  fTrue : typ -> func;
+  fFalse : typ -> func;
+  fAnd : typ -> func;
+  fOr : typ -> func;
+  fImpl : typ -> func;
+  fExists : typ -> typ -> func;
+  fForall : typ -> typ -> func;
+  ilogicS : func -> option (ilfunc typ)
+}.
+    
+Section ILogicFuncSum.
+	Context {typ func : Type} {H : ILogicFunc typ func}.
+
+	Global Instance ILogicFuncSumL (A : Type) : 
+		ILogicFunc typ (func + A) := {
+		  fEntails l := inl (fEntails l);
+		  fTrue l := inl (fTrue l);
+		  fFalse l := inl (fFalse l);
+		  fAnd l := inl (fAnd l);
+		  fOr l := inl (fOr l);
+		  fImpl l := inl (fImpl l);
+		  fExists t l := inl (fExists t l);
+		  fForall t l := inl (fForall t l);
+		  ilogicS f := match f with
+		  				 | inl a => ilogicS a
+		  		   	 	 | _     => None
+		  			   end 
+        }.
+
+	Global Instance ILogicFuncSumR (A : Type) : 
+		ILogicFunc typ (A + func) := {
+		  fEntails l := inr (fEntails l);
+		  fTrue l := inr (fTrue l);
+		  fFalse l := inr (fFalse l);
+		  fAnd l := inr (fAnd l);
+		  fOr l := inr (fOr l);
+		  fImpl l := inr (fImpl l);
+		  fExists t l := inr (fExists t l);
+		  fForall t l := inr (fForall t l);
+		  ilogicS f := match f with
+		  				 | inr a => ilogicS a
+		  		   	 	 | _     => None
+		  			   end 
+        }.
+        
+	Global Instance ILogicFuncExpr : 
+		ILogicFunc typ (expr typ func) := {
+		  fEntails l := Inj (fEntails l);
+		  fTrue l := Inj (fTrue l);
+		  fFalse l := Inj (fFalse l);
+		  fAnd l := Inj (fAnd l);
+		  fOr l := Inj (fOr l);
+		  fImpl l := Inj (fImpl l);
+		  fExists t l := Inj (fExists t l);
+		  fForall t l := Inj (fForall t l);
+		  ilogicS f := match f with
+		  				 | Inj a => ilogicS a
+		  		   	 	 | _     => None
+		  			   end 
+        }.
+
+End ILogicFuncSum.
+
+Section ILogicFuncInst.
+
+	Context {typ func : Type}.
+	Context {HR : RType typ} {Heq : RelDec (@eq typ)} {HC : RelDec_Correct Heq}.
+
+    Variable Typ2_tyArr : Typ2 _ Fun.
+    Variable Typ0_tyProp : Typ0 _ Prop.
+
+    Let tyArr : typ -> typ -> typ := @typ2 _ _ _ _.
+    Let tyProp : typ := @typ0 _ _ _ _.
+
+	Global Instance ILogicFuncInst : ILogicFunc typ (ilfunc typ) := {
+	  fEntails := ilf_entails;
+	  fTrue := ilf_true;
+	  fFalse := ilf_false;
+	  fAnd := ilf_and;
+	  fOr := ilf_or;
+	  fImpl := ilf_impl;
+	  fExists := ilf_exists;
+	  fForall := ilf_forall;
+	  ilogicS f := Some f
+	}.
+
+  Definition logic_ops := forall (t : typ),
+    option (ILogicOps (typD t)).
+  Definition logic_opsOk (l : logic_ops) : Prop :=
+    forall g, match l g return Prop with
+                | Some T => @ILogic _ T
+                | None => True
+              end.
+
+  Variable gs : logic_ops.
+  
+  Definition typeof_ilfunc (f : ilfunc typ) : option typ :=
+    match f with
+      | ilf_true t
+      | ilf_false t => match gs t with
+  				   	     | Some _ => Some t
+				  	     | None => None
+  					   end
+      | ilf_entails t => match gs t with
+					  	   | Some _ => Some (tyArr t (tyArr t tyProp))
+					  	   | None => None
+					   	 end
+      | ilf_and t
+      | ilf_or t
+      | ilf_impl t => match gs t with
+				  	    | Some _ => Some (tyArr t (tyArr t t))
+				  	    | None => None
+				  	  end
+      | ilf_forall a t
+      | ilf_exists a t => match gs t with
+					  	    | Some _ => Some (tyArr (tyArr a t) t)
+					  	    | None => None
+					  	  end
+  	end.
+
+  Global Instance RelDec_ilfunc : RelDec (@eq (ilfunc typ)) :=
+  { rel_dec := fun a b =>
+	         match a, b with
+		   | ilf_entails t, ilf_entails t'
+		   | ilf_true t, ilf_true t'
+		   | ilf_false t, ilf_false t'
+		   | ilf_and t, ilf_and t'
+		   | ilf_or t, ilf_or t'
+		   | ilf_impl t, ilf_impl t' => t ?[eq] t'
+		   | ilf_forall a t, ilf_forall a' t'
+		   | ilf_exists a t, ilf_exists a' t' => (a ?[eq] a' && t ?[eq] t')%bool
+		   | _, _ => false
+	         end
+  }.
+
+  Global Instance RelDec_Correct_ilfunc : RelDec_Correct RelDec_ilfunc.
+  Proof.
+    constructor.
+    destruct x; destruct y; simpl;
+    try solve [ try rewrite Bool.andb_true_iff ;
+                repeat rewrite rel_dec_correct; intuition congruence ].
+  Qed.
+
+  Definition typ2_cast_bin (a b c : typ)
+  : (typD a -> typD b -> typD c) -> typD (tyArr a (tyArr b c)) :=
+    fun f =>
+      match eq_sym (typ2_cast a (tyArr b c)) in _ = t
+            return t with
+        | eq_refl => match eq_sym (typ2_cast b c) in _ = t
+                           return _ -> t with
+                       | eq_refl => f
+                     end
+        end.
+
+  Definition typ2_cast_quant (a b c : typ)
+  : ((typD a -> typD b) -> typD c) -> typD (tyArr (tyArr a b) c) :=
+    fun f =>
+      match eq_sym (typ2_cast (tyArr a b) c) in _ = t
+            return t with
+        | eq_refl => match eq_sym (typ2_cast a b) in _ = t
+                           return t -> _ with
+                       | eq_refl => f
+                     end
+      end.
+ 
+ Definition funcD (f : ilfunc typ) : match typeof_ilfunc f with
+							       | Some t => typD t
+							       | None => unit
+							      end :=
+    match f as f
+          return match typeof_ilfunc f with
+		   | Some t => typD t
+		   | None => unit
+		 end
+    with
+      | ilf_true t => match gs t as x return (match match x with
+											          | Some _ => Some t
+											          | None => None
+											        end with
+				                                 | Some t0 => typD t0
+											 	 | None => unit
+											       end) with
+					    | Some t => @ltrue _ t
+					    | None => tt
+				      end
+      | ilf_false t =>
+        match gs t as x
+              return (match match x with
+			      | Some _ => Some t
+			      | None => None
+			    end with
+			| Some t0 => typD t0
+			| None => unit
+		      end) with
+	  | Some t => @lfalse _ t
+	  | None => tt
+        end
+      | ilf_entails t =>
+        match gs t as x
+              return (match match x with
+			      | Some _ => Some (tyArr t (tyArr t tyProp))
+			      | None => None
+			    end with
+			| Some t0 => typD t0
+			| None => unit
+		      end) with
+	  | Some C =>
+            match eq_sym (typ2_cast t (tyArr t tyProp)) in _ = t
+                  return t with
+              | eq_refl =>
+                match eq_sym (typ2_cast t tyProp) in _ = t
+                      return _ -> t with
+                  | eq_refl =>
+                    match eq_sym (typ0_cast (F := Prop)) in _ = t
+                          return _ -> _ -> t
+                    with
+                      | eq_refl => @lentails _ _
+                    end
+                end
+            end
+	  | None => tt
+        end
+      | ilf_and t =>
+        match gs t as x
+              return (match match x with
+			      | Some _ => Some (tyArr t (tyArr t t))
+			      | None => None
+			    end with
+			| Some t0 => typD t0
+			| None => unit
+		      end) with
+	  | Some t => typ2_cast_bin _ _ _ (@land _ _)
+	  | None => tt
+        end
+      | ilf_impl t =>
+        match gs t as x
+              return (match match x with
+			      | Some _ => Some (tyArr t (tyArr t t))
+			      | None => None
+			    end with
+			| Some t0 => typD t0
+			| None => unit
+		      end) with
+	  | Some t => typ2_cast_bin _ _ _ (@limpl _ _)
+	  | None => tt
+        end
+      | ilf_or t =>
+        match gs t as x
+              return (match match x with
+			      | Some _ => Some (tyArr t (tyArr t t))
+			      | None => None
+			    end with
+			| Some t0 => typD t0
+			| None => unit
+		      end) with
+	  | Some t => typ2_cast_bin _ _ _ (@lor _ _)
+	  | None => tt
+        end
+      | ilf_exists a t =>
+        match gs t as x return (match match x with
+					| Some _ => Some (tyArr (tyArr a t) t)
+					| None => None
+				      end with
+				  | Some t0 => typD t0
+				  | None => unit
+				end) with
+	  | Some t0 => typ2_cast_quant _ _ _ (@lexists _ _ _)
+	  | None => tt
+        end
+      | ilf_forall a t =>
+        match gs t as x return (match match x with
+					| Some _ => Some (tyArr (tyArr a t) t)
+					| None => None
+				      end with
+				  | Some t0 => typD t0
+				  | None => unit
+				end) with
+	  | Some t0 => typ2_cast_quant _ _ _ (@lforall _ _ _)
+	  | None => tt
+        end
+    end.
+
+  Global Instance RSym_ilfunc : SymI.RSym (ilfunc typ) :=
+  { typeof_sym := typeof_ilfunc
+  ; sym_eqb := fun a b => Some (rel_dec a b)
+  ; symD := funcD
+  }.
+
+  Global Instance RSymOk_ilfunc : SymI.RSymOk RSym_ilfunc.
+  Proof.
+    constructor.
+    intros. unfold sym_eqb; simpl.
+    consider (a ?[ eq ] b); auto.
+  Qed.
+
+End ILogicFuncInst.
+
+Section MakeILogic.
+	Context {typ func : Type} {H : ILogicFunc typ func}.
+
+	Definition mkEntails (t : typ) (P Q : expr typ func) := App (App (fEntails t) P) Q.
+	Definition mkTrue t : expr typ func := Inj (fTrue t).
+	Definition mkFalse t : expr typ func := Inj (fFalse t).
+	Definition mkAnd (t : typ) (P Q : expr typ func) := App (App (fAnd t) P) Q.
+	Definition mkOr (t : typ) (P Q : expr typ func) := App (App (fOr t) P) Q.
+	Definition mkImpl (t : typ) (P Q : expr typ func) := App (App (fImpl t) P) Q.
+	Definition mkExists (t l : typ) (f : expr typ func) := App (fExists t l) (Abs t f).
+	Definition mkForall (t l : typ) (f : expr typ func) := App (fForall t l) (Abs t f).
+
+End MakeILogic.
+
+Implicit Arguments RSym_ilfunc [[typ] [HR] [Heq] [Typ2_tyArr] [Typ0_tyProp]].
+
+Section TypeOfFunc.
+  Context {typ func : Type}.
+  Context {RType_typ : RType typ}.
+  Context {RTypeOk_typ : RTypeOk}.
+  Context {RSym_func : RSym func}.
+  
+  Lemma typeof_funcAs f t e (H : funcAs f t = Some e) : typeof_sym f = Some t.
+  Proof.
+    unfold funcAs in H.
+    generalize dependent (symD f).
+    destruct (typeof_sym f); intros; [|congruence].
+    destruct (type_cast t0 t); [|congruence].
+    destruct r; reflexivity.
+  Qed.
+    
+  Lemma funcAs_Some f t (pf : typeof_sym f = Some t) :
+    funcAs f t =
+    Some (match pf in (_ = z)
+      return match z with
+               | Some z' => typD z'
+               | None => unit
+             end
+      with
+      | eq_refl => symD f
+      end).
+  Proof.
+    unfold funcAs.
+    generalize (symD f).
+    rewrite pf. intros.
+    rewrite type_cast_refl. reflexivity. apply _.
+  Qed.
+
+End TypeOfFunc.
+
+Section ILogicFuncOk.
+  Context {typ func : Type} {HO: ILogicFunc typ func}.
+  Context {RType_typ : RType typ} {RSym_func : RSym func}.
+  Context {RelDec_eq : RelDec (@eq typ)}.
+
+  Context {Typ2_tyArr : Typ2 _ Fun}.
+  Context {Typ0_Prop : Typ0 _ Prop}.
+  Let tyArr : typ -> typ -> typ := @typ2 _ _ _ _.
+  
+  Variable gs : logic_ops.
+
+  Class ILogicFuncOk := {
+    ilf_funcAsOk (f : func) e : ilogicS f = Some e -> 
+      forall t, funcAs f t = funcAs (RSym_func := RSym_ilfunc gs) e t;
+    ilf_fEntailsOk t : ilogicS (fEntails t) = Some (ilf_entails t);
+    ilf_fTrueOk t : ilogicS (fTrue t) = Some (ilf_true t);
+    ilf_fFalseOk t : ilogicS (fFalse t) = Some (ilf_false t);
+    ilf_fAndOk t : ilogicS (fAnd t) = Some (ilf_and t);
+    ilf_fOrOk t : ilogicS (fOr t) = Some (ilf_or t);
+    ilf_fImplOk t : ilogicS (fImpl t) = Some (ilf_impl t);
+    ilf_fExistsOk t l : ilogicS (fExists t l) = Some (ilf_exists t l);
+    ilf_fForallOk t l : ilogicS (fForall t l) = Some (ilf_forall t l)
+  }.
+
+End ILogicFuncOk.
+
+Implicit Arguments ILogicFuncOk [[HO] [RType_typ] [RSym_func] [RelDec_eq] [Typ2_tyArr] [Typ0_Prop]].
+
+Section ILogicFuncBaseOk.
+  Context {typ func : Type} {HO: ILogicFunc typ func}.
+  Context {RType_typ : RType typ} {RSym_func : RSym func}.
+  Context {RelDec_eq : RelDec (@eq typ)}.
+
+  Context {Typ2_tyArr : Typ2 _ Fun}.
+  Context {Typ0_Prop : Typ0 _ Prop}.
+  Let tyArr : typ -> typ -> typ := @typ2 _ _ _ _.
+  
+  Variable gs : logic_ops.
+
+  Global Program Instance ILogicFuncBaseOk : ILogicFuncOk (RSym_func := RSym_ilfunc gs) typ (ilfunc typ) gs := {
+    ilf_funcAsOk := fun _ _ _ _ => eq_refl;
+    ilf_fEntailsOk t := eq_refl;
+    ilf_fTrueOk t := eq_refl;
+    ilf_fFalseOk t := eq_refl;
+    ilf_fAndOk t := eq_refl;
+    ilf_fOrOk t := eq_refl;
+    ilf_fImplOk t := eq_refl;
+    ilf_fExistsOk t l := eq_refl;
+    ilf_fForallOk t l := eq_refl
+  }.
+
+End ILogicFuncBaseOk.
+
+Section ILogicFuncExprOk.
+  Context {typ func : Type} `{HOK : ILogicFuncOk typ func}.
+  Context {HROk : RTypeOk}.
+  Context {A : Type} {RSymA : RSym A}.
+
+  Lemma ILogicFunc_typeOk (f : func) (e : ilfunc typ) (H : ilogicS f = Some e) :
+    typeof_sym f = typeof_ilfunc _ _ gs e.
+  Proof.
+    destruct HOK as [H1 H2 _ _ _ _ _ _ _].
+    specialize (H1 _ _ H).
+    destruct e; simpl in *;
+    remember (gs logic) as o;
+    destruct o; try
+    match goal with 
+      | |- typeof_sym ?f = Some ?t => 
+	 	specialize (H1 t);
+	 	simpl in H1;
+	 	unfold funcAs in H1; simpl in H1; rewrite <- Heqo, type_cast_refl in H1; [|apply _];
+	 	generalize dependent (symD f);
+	 	destruct (typeof_sym f); simpl; intros; [forward|]; inversion H1
+ 	end;
+ 	unfold funcAs in H1; simpl in H1; rewrite <- Heqo in H1;
+ 	generalize dependent (symD f);
+ 	remember (typeof_sym f);
+ 	(destruct o; intros; [|reflexivity]);
+ 	specialize (H1 t); (rewrite type_cast_refl in H1; [|apply _]);
+ 	inversion H1. 
+  Qed.
+  
+  Lemma ilogicS_is_ilogic (f : func) (e : ilfunc typ) t df
+  	(H1 : ilogicS f = Some e) (H2 : funcAs f t = Some df) :
+    exists IL, gs (ilfunc_logic e) = Some IL.
+  Proof.
+    pose proof (ilf_funcAsOk _ H1) as H; 
+    rewrite H in H2; clear H;
+    destruct e; simpl in *;
+    unfold funcAs in H2; simpl in H2;
+    (destruct (gs logic); [eexists; reflexivity | congruence]).
+  Qed.
+  
+  Lemma ilf_true_type_eq (f : func) t u df
+    (H1 : ilogicS f = Some (ilf_true t)) (H2 : funcAs f u = Some df) :
+    t = u.
+  Proof.
+    rewrite (ilf_funcAsOk _ H1) in H2.
+    unfold funcAs in H2; simpl in *.
+    forward.
+  Qed.
+
+  Lemma ilf_false_type_eq (f : func) t u df
+    (H1 : ilogicS f = Some (ilf_false t)) (H2 : funcAs f u = Some df) :
+    t = u.
+  Proof.
+    rewrite (ilf_funcAsOk _ H1) in H2.
+    unfold funcAs in H2; simpl in *.
+    forward.
+  Qed.
+
+  Existing Instance RSym_sum.
+
+  Global Program Instance ILogicFuncOkSumR : ILogicFuncOk typ ((A + func)%type) gs := {
+    ilf_funcAsOk := 
+      fun a f H t => 
+        match a with
+          | inl b => _
+          | inr b => _
+        end;
+    ilf_fEntailsOk t := ilf_fEntailsOk (func := func) t;
+    ilf_fTrueOk t := ilf_fTrueOk (func := func) t;
+    ilf_fFalseOk t := ilf_fFalseOk (func := func) t;
+    ilf_fAndOk t := ilf_fAndOk (func := func) t;
+    ilf_fOrOk t := ilf_fOrOk (func := func) t;
+    ilf_fImplOk t := ilf_fImplOk (func := func) t;
+    ilf_fExistsOk t l := ilf_fExistsOk (func := func) t l;
+    ilf_fForallOk t l := ilf_fForallOk (func := func) t l       
+  }.
+  Next Obligation.
+    apply (ilf_funcAsOk (func := func)).
+    apply H.
+  Qed.
+
+  Global Program Instance ILogicFuncOkSumL : ILogicFuncOk typ ((func + A)%type) gs := {
+    ilf_funcAsOk := 
+      fun a f H t => 
+        match a with
+          | inl b => _
+          | inr b => _
+        end;
+    ilf_fEntailsOk t := ilf_fEntailsOk (func := func) t;
+    ilf_fTrueOk t := ilf_fTrueOk (func := func) t;
+    ilf_fFalseOk t := ilf_fFalseOk (func := func) t;
+    ilf_fAndOk t := ilf_fAndOk (func := func) t;
+    ilf_fOrOk t := ilf_fOrOk (func := func) t;
+    ilf_fImplOk t := ilf_fImplOk (func := func) t;
+    ilf_fExistsOk t l := ilf_fExistsOk (func := func) t l;
+    ilf_fForallOk t l := ilf_fForallOk (func := func) t l       
+  }.
+  Next Obligation.
+    apply (ilf_funcAsOk (func := func)).
+    apply H.
+  Qed.
+
+End ILogicFuncExprOk.
+
+Require Import ExtLib.Tactics.
+
+Section MakeILogicSound.
+  Context {typ func : Type} `{HOK : ILogicFuncOk typ func}.
+  Context {HROk : RTypeOk} {Typ2_tyArrOk : Typ2Ok Typ2_tyArr}
+          {RSym_funcOk : RSymOk RSym_func0}.
+
+  Let tyArr : typ -> typ -> typ := @typ2 _ _ _ _.
+
+  Lemma mkTrue_sound (t : typ) (tus tvs : tenv typ) (f : func)
+    (df : typD t)
+    (Ho : ilogicS f = Some (ilf_true t))
+    (Hf : funcAs f t = Some df) :
+    exprD' tus tvs t (mkTrue t) = Some (fun _ _ => df).
+  Proof.
+    unfold mkTrue; simpl.
+    autorewrite with exprD_rw; simpl; forward; inv_all; subst.
+    pose proof (ilf_funcAsOk _ Ho) as H; rewrite H in Hf.
+    pose proof (ilf_fTrueOk t) as H1.
+    pose proof (ilf_funcAsOk _ H1) as H2. rewrite <- H2 in Hf.
+    pose proof (ILogicFunc_typeOk _ H1) as H3. simpl in H3.
+    destruct (ilogicS_is_ilogic _ _ H1 Hf) as [x H4]; simpl in H4; rewrite H4 in H3.
+    rewrite (funcAs_Some _ H3).
+    rewrite (funcAs_Some _ H3) in Hf.
+    inv_all; subst. reflexivity.
+  Qed.
+    
+  Lemma mkFalse_sound (t : typ) (tus tvs : tenv typ) (f : func)
+    (df : typD t)
+    (Ho : ilogicS f = Some (ilf_false t))
+    (Hf : funcAs f t = Some df) :
+    exprD' tus tvs t (mkFalse t) = Some (fun _ _ => df).
+  Proof.
+    unfold mkFalse; simpl.
+    autorewrite with exprD_rw; simpl; forward; inv_all; subst.
+    pose proof (ilf_funcAsOk _ Ho) as H; rewrite H in Hf.
+    pose proof (ilf_fFalseOk t) as H1.
+    pose proof (ilf_funcAsOk _ H1) as H2. rewrite <- H2 in Hf.
+    pose proof (ILogicFunc_typeOk _ H1) as H3. simpl in H3.
+    destruct (ilogicS_is_ilogic _ _ H1 Hf) as [x H4]; simpl in H4; rewrite H4 in H3.
+    rewrite (funcAs_Some _ H3).
+    rewrite (funcAs_Some _ H3) in Hf.
+    inv_all; subst. reflexivity.
+  Qed.
+    
+  Lemma mkAnd_sound (t : typ) (tus tvs : tenv typ) (f : func) p q
+    (df : typD (tyArr t (tyArr t t))) (dp dq : ExprI.exprT tus tvs (typD t))
+    (Ho : ilogicS f = Some (ilf_and t))
+    (Hf : funcAs f (tyArr t (tyArr t t)) = Some df)
+    (Hp : exprD' tus tvs t p = Some dp)
+    (Hq : exprD' tus tvs t q = Some dq) :
+    exprD' tus tvs t (mkAnd t p q) = Some (exprT_App (exprT_App (fun _ _ => df) dp) dq).
+  Proof.
+    unfold mkAnd; simpl.
+    autorewrite with exprD_rw; simpl; forward; inv_all; subst.
+    rewrite (ExprTac.exprD_typeof_Some _ _ _ q _ Hq).
+    autorewrite with exprD_rw; simpl; forward; inv_all; subst.
+    rewrite (ExprTac.exprD_typeof_Some _ _ _ p _ Hp).
+    autorewrite with exprD_rw; simpl; forward; inv_all; subst.
+    pose proof (ilf_funcAsOk _ Ho) as Hfunc; rewrite Hfunc in Hf.
+    pose proof (ilf_fAndOk t) as HfuncOk.
+    pose proof (ilf_funcAsOk _ HfuncOk) as Heq. rewrite <- Heq in Hf.
+    pose proof (ILogicFunc_typeOk _ HfuncOk) as Htype. simpl in Htype.
+    destruct (ilogicS_is_ilogic _ _ HfuncOk Hf) as [x Hgs]; simpl in Hgs; rewrite Hgs in Htype.
+    rewrite (funcAs_Some _ Htype).
+    unfold tyArr in Hf.
+    rewrite (funcAs_Some _ Htype) in Hf.
+    inv_all; subst. reflexivity.
+  Qed.
+    
+  Lemma mkOr_sound (t : typ) (tus tvs : tenv typ) (f : func) p q
+    (df : typD (tyArr t (tyArr t t))) (dp dq : ExprI.exprT tus tvs (typD t))
+    (Ho : ilogicS f = Some (ilf_or t))
+    (Hf : funcAs f (tyArr t (tyArr t t)) = Some df)
+    (Hp : exprD' tus tvs t p = Some dp)
+    (Hq : exprD' tus tvs t q = Some dq) :
+    exprD' tus tvs t (mkOr t p q) = Some (exprT_App (exprT_App (fun _ _ => df) dp) dq).
+  Proof.
+    unfold mkOr; simpl.
+    autorewrite with exprD_rw; simpl; forward; inv_all; subst.
+    rewrite (ExprTac.exprD_typeof_Some _ _ _ q _ Hq).
+    autorewrite with exprD_rw; simpl; forward; inv_all; subst.
+    rewrite (ExprTac.exprD_typeof_Some _ _ _ p _ Hp).
+    autorewrite with exprD_rw; simpl; forward; inv_all; subst.
+    pose proof (ilf_funcAsOk _ Ho) as Hfunc; rewrite Hfunc in Hf.
+    pose proof (ilf_fOrOk t) as HfuncOk.
+    pose proof (ilf_funcAsOk _ HfuncOk) as Heq. rewrite <- Heq in Hf.
+    pose proof (ILogicFunc_typeOk _ HfuncOk) as Htype. simpl in Htype.
+    destruct (ilogicS_is_ilogic _ _ HfuncOk Hf) as [x Hgs]; simpl in Hgs; rewrite Hgs in Htype.
+    rewrite (funcAs_Some _ Htype).
+    unfold tyArr in Hf.
+    rewrite (funcAs_Some _ Htype) in Hf.
+    inv_all; subst. reflexivity.
+  Qed.
+    
+  Lemma mkImpl_sound (t : typ) (tus tvs : tenv typ) (f : func) p q
+    (df : typD (tyArr t (tyArr t t))) (dp dq : ExprI.exprT tus tvs (typD t))
+    (Ho : ilogicS f = Some (ilf_impl t))
+    (Hf : funcAs f (tyArr t (tyArr t t)) = Some df)
+    (Hp : exprD' tus tvs t p = Some dp)
+    (Hq : exprD' tus tvs t q = Some dq) :
+    exprD' tus tvs t (mkImpl t p q) = Some (exprT_App (exprT_App (fun _ _ => df) dp) dq).
+  Proof.
+    unfold mkImpl; simpl.
+    autorewrite with exprD_rw; simpl; forward; inv_all; subst.
+    rewrite (ExprTac.exprD_typeof_Some _ _ _ q _ Hq).
+    autorewrite with exprD_rw; simpl; forward; inv_all; subst.
+    rewrite (ExprTac.exprD_typeof_Some _ _ _ p _ Hp).
+    autorewrite with exprD_rw; simpl; forward; inv_all; subst.
+    pose proof (ilf_funcAsOk _ Ho) as Hfunc; rewrite Hfunc in Hf.
+    pose proof (ilf_fImplOk t) as HfuncOk.
+    pose proof (ilf_funcAsOk _ HfuncOk) as Heq. rewrite <- Heq in Hf.
+    pose proof (ILogicFunc_typeOk _ HfuncOk) as Htype. simpl in Htype.
+    destruct (ilogicS_is_ilogic _ _ HfuncOk Hf) as [x Hgs]; simpl in Hgs; rewrite Hgs in Htype.
+    rewrite (funcAs_Some _ Htype).
+    unfold tyArr in Hf.
+    rewrite (funcAs_Some _ Htype) in Hf.
+    inv_all; subst. reflexivity.
+  Qed.
+(*
+  Lemma mkExists_sound (t a : typ) (tus tvs : tenv typ) (f : func) g
+    (df : typD (tyArr (tyArr a t) t)) (dg : ExprI.exprT tus (a::tvs) (typD t))
+    (Ho : ilogicS f = Some (ilf_exists a t))
+    (Hf : funcAs f (tyArr (tyArr a t) t) = Some df)
+    (Hg : exprD' tus (a::tvs) t g = Some dg) :
+    exprD' tus tvs t (mkExists a t g) = Some (exprT_App (fun _ _ => df) (exprT_Abs dg)).
+  Proof.
+    unfold mkExists; simpl.
+    autorewrite with exprD_rw; simpl; forward; inv_all; subst.
+    rewrite (ExprTac.exprD_typeof_Some _ _ _ g _ Hg).
+    autorewrite with exprD_rw; simpl; forward; inv_all; subst.
+    pose proof (ilf_funcAsOk _ Ho) as Hfunc; rewrite Hfunc in Hf.
+    pose proof (ilf_fExistsOk a t) as HfuncOk.
+    pose proof (ilf_funcAsOk _ HfuncOk) as Heq. rewrite <- Heq in Hf.
+    pose proof (ILogicFunc_typeOk _ HfuncOk) as Htype. simpl in Htype.
+    destruct (ilogicS_is_ilogic _ _ HfuncOk Hf) as [x Hgs]; simpl in Hgs; rewrite Hgs in Htype.
+    unfold tyArr in Hf. rewrite Hf.
+	(* Stuck here *)
+  Qed.
+    *)
+    
+End MakeILogicSound.
