Charge!/src/Charge/ModularFunc/ListFunc.v
@@ -1,0 +1,232 @@
+Require Import ExtLib.Core.RelDec.
+Require Import ExtLib.Data.Fun.
+Require Import ExtLib.Tactics.Consider.
+
+Require Import MirrorCore.TypesI.
+Require Import MirrorCore.syms.SymEnv.
+Require Import MirrorCore.Lambda.Expr.
+
+Require Import Charge.Logics.ILogic.
+Require Import Charge.ModularFunc.ListType.
+Require Import Charge.ModularFunc.BaseType.
+
+Require Import Coq.Strings.String.
+
+Set Implicit Arguments.
+Set Strict Implicit.
+Set Maximal Implicit Insertion.
+
+Inductive list_func (typ : Type) :=
+  | pNil : typ -> list_func typ
+  | pCons : typ -> list_func typ
+  | pLength : typ -> list_func typ
+  | pMap : typ -> typ -> list_func typ
+  | pFold : typ -> typ -> list_func typ
+  | pZip : typ -> typ -> list_func typ.
+
+Class ListFunc (typ func : Type) := {
+  fNil  : typ -> func;
+  fCons : typ -> func;
+  fLength : typ -> func;
+  fMap : typ -> typ -> func;
+  fFold : typ -> typ -> func;
+  fZip : typ -> typ -> func;
+  
+  listS : func -> option (list_func typ)
+}.
+
+Section ListFuncSum.
+	Context {typ func : Type} {H : ListFunc typ func}.
+
+	Global Instance ListFuncSumL (A : Type) : 
+		ListFunc typ (func + A) := {
+		  fNil t := inl (fNil t);
+	      fCons t := inl (fCons t);
+	      fLength t := inl (fLength t);
+          fMap t1 t2 := inl (fMap t1 t2);
+          fFold t1 t2 := inl (fFold t1 t2);
+          fZip t1 t2 := inl (fZip t1 t2);
+          
+          listS f := match f with
+          			   | inl f => listS f
+          			   | inr _ => None
+          			 end
+        }.
+
+	Global Instance ListFuncSumR (A : Type) : 
+		ListFunc typ (A + func) := {
+		  fNil t := inr (fNil t);
+	      fCons t := inr (fCons t);
+	      fLength t := inr (fLength t);
+          fMap t1 t2 := inr (fMap t1 t2);
+          fFold t1 t2 := inr (fFold t1 t2);
+          fZip t1 t2 := inr (fZip t1 t2);
+         
+          listS f := match f with
+          			   | inr f => listS f
+          			   | inl _ => None
+          			 end
+        }.
+
+    Global Instance ListFuncExpr :
+    	ListFunc typ (expr typ func) := {
+    	  fNil t := Inj (fNil t);
+    	  fCons t := Inj (fCons t);
+    	  fLength t := Inj (fLength t);
+    	  fMap t1 t2 := Inj (fMap t1 t2);
+    	  fFold t1 t2 := Inj (fFold t1 t2);
+    	  fZip t1 t2 := Inj (fZip t1 t2);
+         
+          listS f := match f with
+          			   | Inj f => listS f
+          			   | _ => None
+          			 end
+     }.
+        
+End ListFuncSum.
+
+Section ListFuncInst.
+	Context {typ : Type} {HR : RType typ} 
+	        {HTB : BaseType typ} {HTBD : BaseTypeD}
+	        {HT : ListType typ} {HTD: ListTypeD}.
+	Context {func : Type} {H : ListFunc typ func}.
+	Context {Heq : RelDec (@eq typ)} {HC : RelDec_Correct Heq}.
+
+    Variable Typ2_tyArr : Typ2 _ Fun.
+    Variable Typ0_tyProp : Typ0 _ Prop.
+
+    Let tyArr : typ -> typ -> typ := @typ2 _ _ _ _.
+    Let tyProp : typ := @typ0 _ _ _ _.
+
+	Global Instance ListFuncInst : ListFunc typ (list_func typ) := {
+	  fNil := pNil;
+	  fCons := pCons;
+	  fLength := pLength;
+	  fMap := pMap;
+	  fFold := pFold;
+	  fZip := pZip;
+	  
+	  listS f := Some f
+	}.
+
+	Definition typeof_list_func lf :=
+		match lf with
+		  | pNil t => Some (tyList t)
+		  | pCons t => Some (tyArr t (tyArr (tyList t) (tyList t)))
+		  | pLength t => Some (tyArr (tyList t) tyNat)
+		  | pMap t1 t2 => Some (tyArr (tyArr t1 t2) (tyArr (tyList t1) (tyList t2)))
+		  | pFold t1 t2 => Some (tyArr (tyArr t2 (tyArr t1 t1)) (tyArr t1 (tyArr (tyList t2) t1))) 
+		  | pZip t1 t2 => Some (tyArr (tyList t1) (tyArr (tyList t2) (tyList (tyPair t1 t2))))
+		end.
+
+	Definition list_func_eq (a b : list_func typ) : option bool :=
+	  match a , b with
+	    | pNil t1, pNil t2 => Some (t1 ?[ eq ] t2)
+	    | pCons t1, pCons t2 => Some (t1 ?[ eq ] t2)
+	    | pLength t1, pLength t2 => Some (t1 ?[ eq ] t2)
+	    | pMap t1 t2, pMap t3 t4 => Some (t1 ?[ eq ] t3 &&
+	      								    t2 ?[ eq ] t4)%bool
+	    | pFold t1 t2, pFold t3 t4 => Some (t1 ?[ eq ] t3 &&
+	      								    t2 ?[ eq ] t4)%bool
+	    | pZip t1 t2, pZip t3 t4 => Some (t1 ?[ eq ] t3 &&
+	      								    t2 ?[ eq ] t4)%bool
+	    | _, _ => None
+	  end.
+
+    Global Instance RelDec_list_func : RelDec (@eq (list_func typ)) := {
+      rel_dec a b := match list_func_eq a b with 
+    	  		       | Some b => b 
+    		 	       | None => false 
+    			     end
+    }.
+
+	 Definition list_func_symD lf :=
+		match lf as lf return match typeof_list_func lf with
+								| Some t => typD t
+								| None => unit
+							  end with
+	    | pNil t => eq_rect_r id (@nil (typD t)) (btList t)
+	    | pCons t => 
+	       eq_rect_r id
+             (eq_rect_r (fun T : Type => typD t -> T)
+               (fun x xs => 
+                    let xs := eq_rect _ id xs _ (btList t) in
+                    eq_rect_r id (cons x xs) (btList t))
+               (typ2_cast (tyList t) (tyList t)))
+             (typ2_cast t (typ2 (tyList t) (tyList t)))
+	    | pLength t => 
+	        eq_rect_r id 
+	          (fun lst : typD (tyList t) =>
+	    	     let lst := eq_rect (typD (tyList t)) id lst (list (typD t)) (btList t) in
+	    			        eq_rect_r id (List.length lst) btNat)
+	          (typ2_cast (tyList t) (tyNat))
+	    | pMap t1 t2 => 
+	        eq_rect_r id 
+	          (eq_rect_r (fun T : Type => typD (tyArr t1 t2) -> T)
+	            (fun f lst =>
+	              let f := eq_rect _ id f _ (typ2_cast t1 t2) in
+	              let lst := eq_rect _ id lst _ (btList t1) in
+	                eq_rect_r id (List.map f lst) (btList t2))
+	            (typ2_cast (tyList t1) (tyList t2)))
+	          (typ2_cast (tyArr t1 t2) (typ2 (tyList t1) (tyList t2)))
+	    | pFold t1 t2 => 
+	        eq_rect_r id 
+	          (eq_rect_r (fun T : Type => typD (tyArr t2 (tyArr t1 t1)) -> T)
+				(eq_rect_r (fun T : Type => typD (tyArr t2 (tyArr t1 t1)) -> typD t1 -> T)
+					(fun f acc lst =>
+						let f := eq_rect _ id f _ 
+							(eq_ind_r (fun T : Type => T = (typD t2 -> typD t1 -> typD t1))
+						      (eq_ind_r
+						         (fun T : Type => Fun (typD t2) T = (typD t2 -> typD t1 -> typD t1))
+         eq_refl (typ2_cast t1 t1)) (typ2_cast t2 (typ2 t1 t1))) in
+						let lst := eq_rect _ id lst _ (btList t2) in
+						   fold_right f acc lst)
+					(typ2_cast (tyList t2) t1))				  
+	            (typ2_cast t1 (typ2 (tyList t2) t1)))
+	          (typ2_cast (typ2 t2 (typ2 t1 t1)) (typ2 t1 (typ2 (tyList t2) t1)))
+	    | pZip t1 t2 => 
+	        eq_rect_r id 
+	          (eq_rect_r (fun T : Type => typD (tyList t1) -> T)
+	            (fun xs ys =>
+	              let xs := eq_rect _ id xs _ (btList t1) in
+	              let ys := eq_rect _ id ys _ (btList t2) in
+	                eq_rect_r id (combine xs ys) 
+	                  (eq_ind_r (fun T => T = list ((typD t1 * typD t2)%type))
+	                    (eq_ind_r (fun T => list T = list ((typD t1 * typD t2)%type)) eq_refl
+	                  	  (btPair t1 t2))
+	                  	(btList (tyPair t1 t2))))
+	            (typ2_cast (tyList t2) (tyList (tyPair t1 t2))))
+	          (typ2_cast (tyList t1) (typ2 (tyList t2) (tyList (tyPair t1 t2))))
+	 end.
+
+	Global Instance RSym_ListFunc : SymI.RSym (list_func typ) := {
+	  typeof_sym := typeof_list_func;
+	  symD := list_func_symD;
+	  sym_eqb := list_func_eq
+	}.
+
+	Global Instance RSymOk_ListFunc : SymI.RSymOk RSym_ListFunc.
+	Proof.
+		split; intros.
+		destruct a, b; simpl; try apply I.
+		+ consider (t ?[ eq ] t0); intuition congruence.
+		+ consider (t ?[ eq ] t0); intuition congruence.
+		+ consider (t ?[ eq ] t0); intuition congruence.
+		+ consider (t ?[ eq ] t1 && t0 ?[ eq ] t2)%bool; intuition congruence. 
+		+ consider (t ?[ eq ] t1 && t0 ?[ eq ] t2)%bool; intuition congruence. 
+		+ consider (t ?[ eq ] t1 && t0 ?[ eq ] t2)%bool; intuition congruence. 
+	Qed.
+
+End ListFuncInst.
+
+Section MakeList.
+	Context {typ func : Type} {H : ListFunc typ func}.
+
+	Definition mkNil t : expr typ func := Inj (fNil t).
+	Definition mkCons (t : typ) (x xs : expr typ func) := App (App (fCons t) x) xs.
+	Definition mkLength (t : typ) (lst : expr typ func) := App (fLength t) lst.
+	Definition mkMap (t u : typ) (f lst : expr typ func) :=  App (App (fMap t u) f) lst.
+	Definition mkFold (t u : typ) (f acc lst : expr typ func) :=  App (App (App (fFold t u) f) acc) lst.
+	Definition mkZip (t u : typ) (xs ys : expr typ func) := App (App (fZip t u) xs) ys.
+	
+End MakeList.
