Charge!/src/Charge/ModularFunc/OpenFunc.v
@@ -1,0 +1,810 @@
+Require Import ExtLib.Core.RelDec.
+Require Import ExtLib.Structures.Applicative.
+Require Import ExtLib.Data.Fun.
+Require Import ExtLib.Data.String.
+Require Import ExtLib.Tactics.Consider.
+Require Import ExtLib.Tactics.
+
+Require Import MirrorCore.TypesI.
+Require Import MirrorCore.syms.SymEnv.
+Require Import MirrorCore.Lambda.Expr.
+Require Import MirrorCore.Lambda.ExprVariables.
+Require Import MirrorCore.Lambda.ExprTac.
+Require Import MirrorCore.SymI.
+Require Import MirrorCore.syms.SymSum.
+
+Require Import Charge.Open.Stack.
+Require Import Charge.Open.Subst.
+Require Import Charge.ModularFunc.BaseType.
+Require Import Charge.ModularFunc.ListType.
+Require Import Charge.ModularFunc.SubstType.
+Require Import Charge.ModularFunc.ListFunc.
+Require Import Charge.ModularFunc.ILogicFunc.
+Require Import Charge.ModularFunc.BILogicFunc.
+Require Import Charge.ModularFunc.BaseFunc.
+Require Import Charge.ModularFunc.EmbedFunc.
+Require Import Charge.Rel.
+
+Require Import Coq.Strings.String.
+Require Import Coq.Bool.Bool.
+Require Import FunctionalExtensionality.
+
+Set Implicit Arguments.
+Set Strict Implicit.
+Set Maximal Implicit Insertion.
+
+  Inductive open_func typ {RType_typ : RType typ} {HST : SubstType typ} :=
+    | of_const (_ : typ)
+    | of_ap (_ _ : typ)
+    | of_null
+    | of_stack_get
+    | of_stack_set
+    | of_apply_subst (_ : typ)
+    | of_single_subst
+    | of_subst
+    | of_trunc_subst.
+    
+Implicit Arguments open_func [[RType_typ] [HST]].
+    
+Class OpenFunc (typ func : Type) {RType_typ : RType typ} {HST : SubstType typ} := {
+  fConst : typ -> func;
+  fAp : typ -> typ -> func;
+  
+  fNull : func;
+  
+  fStackGet : func;
+  fStackSet : func;
+  
+  fApplySubst : typ -> func;
+  fSingleSubst : func;
+  fSubst : func;
+  fTruncSubst : func;
+  
+  open_funcS : func -> option (open_func typ)
+}.
+
+Implicit Arguments OpenFunc [[RType_typ] [HST]].
+
+Section OpenFuncSum.
+	Context {typ func : Type} `{H : OpenFunc typ func}.
+
+	Global Instance OpenFuncSumL (A : Type) : 
+	   OpenFunc typ (func + A) := {
+		  fConst t := inl (fConst t);
+		  fAp t u := inl (fAp t u);
+		  
+		  fNull := inl fNull;
+		  
+		  fStackGet := inl fStackGet;
+		  fStackSet := inl fStackSet;
+		  
+		  fApplySubst t := inl (fApplySubst t);
+		  fSingleSubst := inl fSingleSubst;
+		  fSubst := inl fSubst;
+		  fTruncSubst := inl fTruncSubst;
+		  
+		  open_funcS f := match f with
+		  				    | inl f => open_funcS f
+		  				    | inr _ => None
+		  				  end
+       }.
+
+	Global Instance OpenFuncSumR (A : Type) : 
+	   OpenFunc typ (A + func) := {
+		  fConst t := inr (fConst t);
+		  fAp t u := inr (fAp t u);
+		  
+		  fNull := inr fNull;
+		  
+		  fStackGet := inr fStackGet;
+		  fStackSet := inr fStackSet;
+		  
+		  fApplySubst t := inr (fApplySubst t);
+		  fSingleSubst := inr fSingleSubst;
+		  fSubst := inr fSubst;
+		  fTruncSubst := inr fTruncSubst;
+		  
+		  open_funcS f := match f with
+		  				    | inr f => open_funcS f
+		  				    | inl _ => None
+		  				  end
+		  
+       }.
+
+	Global Instance OpenFuncExpr : 
+	   OpenFunc typ (expr typ func) := {
+		  fConst t := Inj (fConst t);
+		  fAp t u := Inj (fAp t u);
+		  
+		  fNull := Inj fNull;
+		  
+		  fStackGet := Inj fStackGet;
+		  fStackSet := Inj fStackSet;
+		  
+		  fApplySubst t := Inj (fApplySubst t);
+		  fSingleSubst := Inj fSingleSubst;
+		  fSubst := Inj fSubst;
+		  fTruncSubst := Inj fTruncSubst;
+		  
+		  open_funcS f := match f with
+		  				    | Inj f => open_funcS f
+		  				    | _ => None
+		  				  end
+		  
+       }.
+
+End OpenFuncSum.
+
+Section OpenFuncInst.
+
+	Context {typ func : Type} {HBT : BaseType typ} {HLT : ListType typ}.
+	Context {HR : RType typ} {Heq : RelDec (@eq typ)} {HC : RelDec_Correct Heq}.
+
+    Variable Typ2_tyArr : Typ2 _ Fun.
+    Variable Typ0_tyProp : Typ0 _ Prop.
+    
+    Context {HST : SubstType typ} {HV : ValNull (typD tyVal)}.
+    Context {HSTD : SubstTypeD}.
+    Context {HBTD : BaseTypeD} {HLTD : ListTypeD}.
+    
+	Context {RelDec_string : RelDec (@eq (typD tyString))}.
+	Context {RelDec_string_Correct : RelDec_Correct RelDec_string}.
+	
+    Let tyArr : typ -> typ -> typ := @typ2 _ _ _ _.
+    Let tyProp : typ := @typ0 _ _ _ _.
+
+	Local Notation "'tyStack'" := (tyArr tyString tyVal).
+	Local Notation "'tyExpr'" := (tyArr tyStack tyVal).
+	Local Notation "'tySubstList'" := (tyList (tyPair tyString (tyArr tyStack tyVal))).
+
+	Definition stack := @stack (typD tyString) (typD tyVal).
+
+	Global Instance OpenFuncInst : OpenFunc typ (open_func typ) := {
+	  fConst := of_const;
+	  fAp := of_ap;
+	  fNull := of_null;
+	  fStackGet := of_stack_get;
+	  fStackSet := of_stack_set;
+	  fApplySubst := of_apply_subst;
+	  fSingleSubst := of_single_subst;
+	  fSubst := of_subst;
+	  fTruncSubst := of_trunc_subst;
+	  
+	  open_funcS f := Some f
+	}.
+  
+  Definition typeof_open_func (f : open_func typ) : option typ :=
+    match f with
+    | of_const t => Some (tyArr t (tyArr tyStack t))
+    | of_ap t u => Some (tyArr (tyArr tyStack (tyArr t u)) (tyArr (tyArr tyStack t) (tyArr tyStack u)))
+    | of_apply_subst t => Some (tyArr (tyArr tyStack t) (tyArr tySubst (tyArr tyStack t)))
+	| of_null => Some tyVal
+    | of_stack_get => Some (tyArr tyString tyExpr)
+    | of_stack_set => Some (tyArr tyString (tyArr tyVal (tyArr tyStack tyStack)))
+    | of_single_subst => Some (tyArr tyExpr (tyArr tyString tySubst))
+    | of_subst => Some (tyArr tySubstList tySubst)
+    | of_trunc_subst => Some (tyArr tySubstList tySubst)
+	end.
+
+  Global Instance RelDec_open_func : RelDec (@eq (open_func typ)) :=
+  { rel_dec := fun a b =>
+	         match a, b with
+	  	       | of_const t, of_const t'
+	  	       | of_apply_subst t, of_apply_subst t' => t ?[eq] t'
+	  	       | of_ap t u, of_ap t' u' => (t ?[eq] t' && u ?[eq] u')%bool
+	  	       | of_null, of_null
+	  	       | of_stack_get, of_stack_get
+	  	       | of_stack_set, of_stack_set
+	  	       | of_single_subst, of_single_subst
+	  	       | of_subst, of_subst
+	  	       | of_trunc_subst, of_trunc_subst => true
+	  	       | _, _ => false
+	         end
+  }.
+
+  Global Instance RelDec_Correct_open_func : RelDec_Correct RelDec_open_func.
+  Proof.
+    constructor.
+    destruct x; destruct y; simpl; try rewrite andb_true_iff;
+    repeat rewrite rel_dec_correct; try intuition congruence.
+  Qed.
+  
+	Local Instance Applicative_Fun A : Applicative (Fun A) :=
+	{ pure := fun _ x _ => x
+	; ap := fun _ _ f x y => (f y) (x y)
+	}.
+
+  Definition fun_to_typ {a b : typ} (f : typD a -> typD b) : typD (tyArr a b) :=
+    eq_rect_r id f (typ2_cast a b).
+    
+  Definition typ_to_fun {a b : typ} (f : typD (tyArr a b)) : typD a -> typD b :=
+  fun x => (fun g : typD a -> typD b => g x)
+    (eq_rect (typD (typ2 a b)) id f (typD a -> typD b)
+       (typ2_cast a b)).
+    
+Definition fun_to_typ2 {a b c : typ} (f : typD a -> typD b -> typD c) :=
+   fun_to_typ (fun x => fun_to_typ (f x)). 
+
+Definition fun_to_typ3 {a b c d : typ} (f : typD a -> typD b -> typD c -> typD d) :=
+  fun_to_typ (fun x => fun_to_typ (fun y => fun_to_typ (f x y))).
+
+Definition typ_to_fun2 {a b c : typ} (f : typD (tyArr a (tyArr b c))) : typD a -> typD b -> typD c :=
+  fun x => typ_to_fun (typ_to_fun f x).
+
+Definition typ_to_fun3 {a b c d : typ} (f : typD (tyArr a (tyArr b (tyArr c d)))) : 
+	typD a -> typD b -> typD c -> typD d :=
+  fun x y => typ_to_fun (typ_to_fun (typ_to_fun f x) y).
+
+
+  Definition fun1_wrap {a b : typ} (f : typD a -> typD b) :=
+      eq_rect_r id f (typ2_cast a b).
+  
+  Definition fun1D {a b : typ} (f : typD (tyArr a b)) (x : typD a) : typD b :=
+  (fun g : typD a -> typD b => g x)
+    (eq_rect (typD (typ2 a b)) id f (typD a -> typD b)
+       (typ2_cast a b)).
+        
+  Definition fun2_wrap {a b c : typ} (f : typD a -> typD b -> typD c) : typD (tyArr a (tyArr b c)) :=
+    fun1_wrap (fun x => fun1_wrap (fun y : typD b => f x y)).
+  
+  Definition fun2D {a b c : typ} (f : typD (tyArr a (tyArr b c))) (x : typD a) (y : typD b) : typD c :=
+    (fun g : typD a -> typD (typ2 b c) =>
+      (fun h : typD a -> typD b -> typD c => h x y)
+        (eq_rect (typD (typ2 b c)) (fun T : Type => typD a -> T) g
+          (typD b -> typD c) (typ2_cast b c)))
+      (eq_rect (typD (typ2 a (typ2 b c))) id f
+         (typD a -> typD (typ2 b c)) (typ2_cast a (typ2 b c))).
+  
+  Definition fun3_wrap {a b c d : typ} (f : typD a -> typD b -> typD c -> typD d) :  
+   typD (tyArr a (tyArr b (tyArr c d))) :=
+     fun1_wrap (fun x => fun2_wrap (fun y z => f x y z)).
+
+  Definition fun4_wrap {a b c d e : typ} (f : typD a -> typD b -> typD c -> typD d -> typD e) :  
+   typD (tyArr a (tyArr b (tyArr c (tyArr d e)))) :=
+     fun1_wrap (fun x => fun3_wrap (fun y z z' => f x y z z')).
+
+(*
+	 Program Definition open_func_symD bf :=
+		match bf as bf return match typeof_open_func bf with
+								| Some t => typD t
+								| None => unit
+							  end with
+	    | of_cons t => typ2_cast_bin t tyStack t 
+	    	(eq_rect_r (fun T : Type => typD t -> T -> typD t) 
+	    		(@pure (Fun stack) (Applicative_Fun _) (typD t)) (typ2_cast d r))
+  				
+	    | of_ap t u => _
+	    | of_stack_set => _
+	    | of_stack_get => _
+	    | of_apply_subst t => _
+	    | of_subst => _
+	    | of_trunc_subst => _
+	 end.
+	 Next Obligation.
+		apply typ3_cast_bin.
+		unfold tyArr. repeat rewrite typ2_cast. unfold Fun.
+		apply (@Applicative.ap (Fun stack) (Applicative_Fun _) (typD t) (typD u)).
+	 Defined.
+	 Next Obligation.
+	    apply typ2_cast_bin.
+	    unfold tyArr. rewrite typ2_cast.
+	    apply (fun (x : typD d) (s : stack) => s x).
+	 Defined.
+	 Next Obligation.
+	 	unfold tyArr; repeat rewrite typ2_cast; unfold Fun.
+	 	pose (@stack_add (typD d) _ (@VN typ _ r null)). apply s.
+	 Defined.
+	 Next Obligation.
+		unfold tyArr; repeat rewrite typ2_cast; unfold Fun.
+		rewrite stSubst.
+		apply (@apply_subst (typD d) (@VN typ _ r null) (typD t)).
+	 Defined.
+	 Next Obligation.
+	    unfold tyArr; rewrite typ2_cast; unfold Fun.
+	    rewrite btList, btPair, stSubst; repeat rewrite typ2_cast.
+	    apply (@substl_aux (typD d) _ (@VN typ _ r null)).
+	 Defined.
+	 Next Obligation.
+		unfold tyArr; rewrite typ2_cast; unfold Fun.
+		rewrite btList, btPair, stSubst. repeat rewrite typ2_cast.
+		apply (@substl_trunc_aux (typD d) _ (@VN typ _ r null)).
+	 Defined.
+*)
+
+	    Definition substListD (lst : typD tySubstList) : substlist (A := typD tyString) (val := (typD tyVal)).
+	    Proof.
+	      rewrite btList, btPair, btString in lst.
+	      unfold tyArr in lst.
+	      repeat rewrite typ2_cast in lst.
+	      rewrite btString in lst.
+	      rewrite btString.
+	      apply lst.
+	   Defined.
+
+	 Definition open_func_symD f : match typeof_open_func f with
+	                                 | Some t => typD t
+	                                 | None => unit
+	                               end :=
+		match f as f return match typeof_open_func f with
+								| Some t => typD t
+								| None => unit
+							  end with
+	      | of_const t =>
+	        fun2_wrap
+		      (eq_rect_r (fun T : Type => typD t -> T -> typD t) pure
+		         (typ2_cast tyString tyVal))
+	      | of_ap t1 t2 => 
+	        fun3_wrap 
+	          (fun a b c => @ap (Fun (typD tyStack)) (Applicative_Fun _) (typD t1) (typD t2)
+	            (fun2D a)
+	            (fun1D b)
+	            c)
+	      | of_null => null
+	      | of_stack_get => fun2_wrap (fun x s => (fun1D s) x)
+	      | of_stack_set => 
+	        (fun4_wrap
+	          (fun a b c d => stack_add a b (fun1D c) d))
+	      | of_apply_subst t => fun_to_typ3
+	         (fun a b c => apply_subst 
+	           (fun x => typ_to_fun a (fun_to_typ x))
+	           (eq_rect (typD tySubst) id b subst stSubst)
+	           (typ_to_fun c))
+	      | of_single_subst => 
+	        fun2_wrap (fun a b => eq_rect_r id (subst1 (fun x => fun1D a (fun1_wrap x)) b) stSubst)
+	      | of_subst => 
+	        fun1_wrap 
+	          (fun a => eq_rect_r id 
+	            (substl_aux (substListD a)) stSubst)
+	      | of_trunc_subst =>
+	        fun1_wrap 
+	          (fun a => eq_rect_r id 
+	            (substl_trunc_aux (substListD a)) stSubst)
+	    end.
+
+	Global Program Instance RSym_OpenFunc : SymI.RSym (open_func typ) := {
+	  typeof_sym := typeof_open_func;
+	  symD := open_func_symD;
+	  sym_eqb := (fun a b => Some (rel_dec a b))
+	}.
+
+  Global Instance RSymOk_lopen_func : SymI.RSymOk RSym_OpenFunc.
+  Proof.
+    constructor.
+    intros. unfold sym_eqb; simpl.
+    consider (a ?[ eq ] b); auto.
+  Qed.
+
+End OpenFuncInst.
+
+Section OpenFuncOk.
+  Context {typ func : Type} {HBT : BaseType typ} {HLT : ListType typ} {HST : SubstType typ}.
+  Context {HR : RType typ} {HO: OpenFunc typ func} {Heq' : RelDec (@eq typ)}. 
+  Context {HS : RSym func} {Heq : RelDec (@eq (typD tyString))}.
+  Context {HV : ValNull (typD tyVal)}.
+
+  Context {HSTD : SubstTypeD}.
+  Context {HBTD : BaseTypeD} {HLTD : ListTypeD}.
+
+  Context  {Typ2_tyArr : Typ2 _ Fun}.
+  Let tyArr : typ -> typ -> typ := @typ2 _ _ _ _.
+
+  Class OpenFuncOk := {
+    of_funcAsOk f e : open_funcS f = Some e -> forall t, funcAs f t = funcAs e t;
+    of_fConstOk t : open_funcS (fConst t) = Some (of_const t);
+    of_fApOk t u : open_funcS (fAp t u) = Some (of_ap t u);
+    of_fNullOk : open_funcS fNull = Some of_null;
+    of_fStackGetOk : open_funcS fStackGet = Some of_stack_get;
+    of_fStackSetOk : open_funcS fStackSet = Some of_stack_set;
+    of_fApplySubstOk t : open_funcS (fApplySubst t) = Some (of_apply_subst t);
+    of_fSingleSubstOk : open_funcS fSingleSubst = Some of_single_subst;
+    of_fSubstOk : open_funcS fSubst = Some of_subst;
+    of_fTruncSubstOk : open_funcS fTruncSubst = Some of_trunc_subst
+  }.
+
+End OpenFuncOk.
+
+Implicit Arguments OpenFuncOk [[HBT] [HLT] [HST] [HR] [HO] [Heq'] [HS] [Heq] [HV] [HSTD] [HBTD] [HLTD] [Typ2_tyArr]].
+
+Section OpenFuncBaseOk.
+  Context {typ func : Type} {HBT : BaseType typ} {HLT : ListType typ} {HST : SubstType typ}.
+  Context {HR : RType typ} {HO: OpenFunc typ func} {Heq' : RelDec (@eq typ)}. 
+  Context {HS : RSym func} {Heq : RelDec (@eq (typD tyString))}.
+  Context {HV : ValNull (typD tyVal)}.
+
+  Context {HSTD : SubstTypeD}.
+  Context {HBTD : BaseTypeD} {HLTD : ListTypeD}.
+
+  Context  {Typ2_tyArr : Typ2 _ Fun}.
+  Let tyArr : typ -> typ -> typ := @typ2 _ _ _ _.
+
+  Program Instance open_funcOk : OpenFuncOk typ (open_func typ) := {
+    of_funcAsOk := fun _ _ _ _ => eq_refl;
+    of_fConstOk t := eq_refl;
+    of_fApOk t u := eq_refl;
+    of_fNullOk := eq_refl;
+    of_fStackGetOk := eq_refl;
+    of_fStackSetOk := eq_refl;
+    of_fApplySubstOk t := eq_refl;
+    of_fSingleSubstOk := eq_refl;
+    of_fSubstOk := eq_refl;
+    of_fTruncSubstOk := eq_refl
+  }.
+  
+End OpenFuncBaseOk.
+
+Section OpenFuncExprOk.
+  Context {typ func : Type} `{HOK : OpenFuncOk typ func}.
+  Context {HROk : RTypeOk}.
+
+  Lemma open_funcSome (f : func) (e : open_func typ) (t : typ)
+    (H : open_funcS f = Some e) : 
+      match typeof_open_func _ e with
+        | Some t => funcAs f t <> None
+        | None => False
+      end.
+  Proof.
+    destruct HOK as [H1].
+    specialize (H1 _ _ H).
+    destruct e; simpl in *; intros H2;
+    match goal with 
+      | H : funcAs _ ?t = None |- _ => 
+        specialize (H1 t); rewrite H in H1; clear H;
+              unfold funcAs in H1; simpl in H1; 
+              rewrite type_cast_refl in H1; [|apply _]; inversion H1
+    end.
+  Qed.
+
+  Lemma OpenFunc_typeOk (f : func) (e : open_func typ) (H : open_funcS f = Some e) :
+    typeof_sym f = typeof_open_func _ e.
+  Proof.
+    destruct HOK as [H1].
+    specialize (H1 _ _ H).
+ 	destruct e; simpl in *;
+    match goal with 
+      | |- typeof_sym ?f = Some ?t => 
+	 	specialize (H1 t);
+	 	simpl in H1;
+ 	 	unfold funcAs in H1; simpl in H1; rewrite type_cast_refl in H1; [|apply _];
+ 		generalize dependent (symD f);
+ 		destruct (typeof_sym f); simpl; intros; [forward|]; inversion H1
+    end.
+  Qed.
+
+  Existing Instance RSym_sum.
+  Existing Instance RSymOk_sum.
+
+  Context {A : Type} {RSymA : RSym A}.
+
+
+  Global Program Instance OpenFuncOkSumR : OpenFuncOk typ (A + func) := {
+    of_funcAsOk := 
+      fun a f H t => 
+        match a with
+          | inl b => _
+          | inr b => _
+        end;
+    of_fConstOk t := of_fConstOk t (func := func);
+    of_fApOk t u := of_fApOk t u (func := func);
+    of_fNullOk := of_fNullOk (func := func);
+    of_fStackGetOk := of_fStackGetOk (func := func);
+    of_fStackSetOk := of_fStackSetOk (func := func);
+    of_fApplySubstOk t := of_fApplySubstOk t (func := func);
+    of_fSingleSubstOk := of_fSingleSubstOk (func := func);
+    of_fSubstOk := of_fSubstOk (func := func);
+    of_fTruncSubstOk := of_fTruncSubstOk (func := func)
+  }.
+  Next Obligation.
+    apply (of_funcAsOk _ H).
+  Qed.
+
+  Global Program Instance OpenFuncOkSumL : OpenFuncOk typ (func + A) := {
+    of_funcAsOk := 
+      fun a f H t => 
+        match a with
+          | inl b => _
+          | inr b => _
+        end;
+    of_fConstOk t := of_fConstOk t (func := func);
+    of_fApOk t u := of_fApOk t u (func := func);
+    of_fNullOk := of_fNullOk (func := func);
+    of_fStackGetOk := of_fStackGetOk (func := func);
+    of_fStackSetOk := of_fStackSetOk (func := func);
+    of_fApplySubstOk t := of_fApplySubstOk t (func := func);
+    of_fSingleSubstOk := of_fSingleSubstOk (func := func);
+    of_fSubstOk := of_fSubstOk (func := func);
+    of_fTruncSubstOk := of_fTruncSubstOk (func := func)
+  }.
+  Next Obligation.
+    apply (of_funcAsOk _ H).
+  Qed.
+  
+End OpenFuncExprOk.
+
+Section MakeOpen.
+	Context {typ func : Type} {HR : RType typ} {HS : SubstType typ}.
+	Context {H : OpenFunc typ func} {H1 : ListFunc typ func}
+	        {HBT : BaseType typ}.
+
+    Context  {Typ2_tyArr : Typ2 _ Fun}.
+    Let tyArr : typ -> typ -> typ := @typ2 _ _ _ _.
+
+	Local Notation "'tyStack'" := (tyArr tyString tyVal).
+
+    Definition mkNull : expr typ func := Inj fNull.
+	Definition mkConst (t : typ) (e : expr typ func) := App (fConst t) e.
+	Definition mkAp (t u : typ) (f e : expr typ func) := App (App (fAp t u) f) e.
+	Definition mkStackGet (x s : expr typ func) := App (App fStackGet x) s.
+	Definition mkStackSet (x v s : expr typ func) := App (App (App fStackSet x) v) s.
+	Definition mkApplySubst (t : typ) (P s : expr typ func) := App (App (fApplySubst t) P) s.
+	Definition mkSingleSubst (e x : expr typ func) := App (App fSingleSubst e) x.
+	Definition mkApplySingleSubst t P x e := mkApplySubst t P (mkSingleSubst x e).	
+	Definition mkSubst (s : expr typ func) := App fSubst s.
+	Definition mkTruncSubst (s : expr typ func) := App fTruncSubst s.
+	Definition mkApplyTruncSubst t P s := mkApplySubst t P (mkTruncSubst s).
+			
+	Fixpoint mkAps f es t :=
+		match es with 
+			| nil => mkConst t f
+			| (e, t')::es => mkAp t' t (mkAps f es (tyArr t' t)) e
+		end.
+
+	Context {HSf : RSym func}.
+(*
+	Fixpoint ap_lift_aux tus tvs (e : expr typ func) (t : typ) : option (expr typ func) :=
+	  match e with
+		| App f a => 
+		  match typeof_expr tus tvs a with
+		    | Some u => 
+		        match ap_lift_aux tus tvs f (tyArr u t), ap_lift_aux tus tvs a u with
+		    	  | Some f', Some a' => Some (mkAp u t f' a')
+		    	  | _, _ => None
+		    	end		
+		    | None => None
+		  end
+		| Inj f => Some (mkConst t (Inj f))
+		| Abs u f => match (ap_lift_aux tus (u::tvs) f (tyArr u t)) with
+					   | Some f' => Some (Abs (tyArr tyStack u) f')
+					   | None => None
+					 end
+						
+		| _ => Some e
+	  end.
+
+	Definition ap_lift2 tus tvs (e : expr typ func) :=
+		match typeof_expr tus tvs e with
+		  | Some t => ap_lift_aux tus tvs e t
+		  | None => None
+		end.
+*)
+
+	Context {HIL : ILogicFunc typ func}.
+	Context {HBIL : BILogicFunc typ func}.
+
+	Fixpoint il_lift tus tvs (e : expr typ func) :=
+	  match e with
+	    | App (App f a) b => 
+	      match ilogicS f with
+	        | Some (ilf_entails t) =>
+	          match il_lift tus tvs a, il_lift tus tvs b with
+	            | Some a', Some b' => Some (mkEntails (tyArr tyStack t) a' b')
+	            | _, _ => None
+	          end
+	        | Some (ilf_and t) =>
+	          match il_lift tus tvs a, il_lift tus tvs b with
+	            | Some a', Some b' => Some (mkAnd (tyArr tyStack t) a' b')
+	            | _, _ => None
+	          end
+	        | Some (ilf_or t) =>
+	          match il_lift tus tvs a, il_lift tus tvs b with
+	            | Some a', Some b' => Some (mkOr (tyArr tyStack t) a' b')
+	            | _, _ => None
+	          end
+	        | Some (ilf_impl t) =>
+	          match il_lift tus tvs a, il_lift tus tvs b with
+	            | Some a', Some b' => Some (mkImpl (tyArr tyStack t) a' b')
+	            | _, _ => None
+	          end
+	        | _ => 
+	          match bilogicS f with
+	            | Some (bilf_star t) =>
+		          match il_lift tus tvs a, il_lift tus tvs b with
+		            | Some a', Some b' => Some (mkStar (tyArr tyStack t) a' b')
+		            | _, _ => None
+		          end
+	            | Some (bilf_wand t) =>
+		          match il_lift tus tvs a, il_lift tus tvs b with
+		            | Some a', Some b' => Some (mkWand (tyArr tyStack t) a' b')
+		            | _, _ => None
+		          end
+	            | _ => 
+	              match typeof_expr tus tvs e, typeof_expr tus tvs a, typeof_expr tus tvs b with
+	                | Some t, Some u, Some v =>
+	            	  match il_lift tus tvs f, il_lift tus tvs a, il_lift tus tvs b with
+	            	    | Some f', Some a', Some b' =>
+	            	      Some (mkAp v t (mkAp u (tyArr v t) f' a') b')
+	            	    | _, _, _ => None 
+	            	  end
+	            	| _, _, _ => None
+	              end
+	          end
+	      end
+	    | App f a =>
+	      match ilogicS f with
+	        | Some (ilf_exists u v) =>
+	          match il_lift tus tvs a with
+	            | Some a' => Some (App (fExists (tyArr tyStack u) (tyArr tyStack v)) a')
+	            | None => None
+	          end
+	        | Some (ilf_forall u v) =>
+	          match il_lift tus tvs a with
+	            | Some a' => Some (App (fForall (tyArr tyStack u) (tyArr tyStack v)) a')
+	            | None => None
+	          end
+	        | _ =>
+	          match typeof_expr tus tvs e, typeof_expr tus tvs a with
+	            | Some t, Some u =>
+	              match il_lift tus tvs f, il_lift tus tvs a with
+	                | Some f', Some a' => Some (mkAp u t f' a')
+	                | _, _ => None
+	              end 
+	            | _, _ => None
+	          end
+	      end
+	    | Inj f =>
+	      match ilogicS f with
+	        | Some (ilf_true t) => Some (mkTrue (tyArr tyStack t))
+	        | Some (ilf_false t) => Some (mkFalse (tyArr tyStack t))
+	        | _ => 
+	          match bilogicS f with
+	            | Some (bilf_emp t) => Some (mkEmp (tyArr tyStack t))
+	            | _ =>
+	              match typeof_expr tus tvs e with
+	                | Some t => Some (mkConst t e)
+	                | None => None
+	              end
+	          end
+	      end
+		| Abs t f => 
+		  match il_lift tus (t::tvs) f with
+		    | Some f' => Some (Abs (tyArr tyStack t) f')
+		    | None => None
+		  end
+	    | _ => Some e
+	  end.
+(*	   
+	with ap_lift tus tvs (e : expr typ func) {struct e} :=
+		match e with
+		  | Abs t f => 
+		    match il_lift tus (t::tvs) f with
+		      | Some f' => Some (Abs (tyArr tyStack t) f')
+		      | None => None
+		    end
+		  | Inj f =>
+		    match typeof_expr tus tvs e with
+		      | Some t => Some (mkConst t (Inj f))
+		      | None => None
+		    end
+		  | App f a =>
+		    match typeof_expr tus tvs e, typeof_expr tus tvs a with
+		      | Some t, Some u =>
+		        match il_lift tus tvs f, il_lift tus tvs a with
+		          | Some f', Some a' => Some (mkAp u t f' a')
+		          | _, _ => None
+		        end
+		      | _, _ => None
+		    end 
+		  | _ => Some e
+		end.
+*)	
+End MakeOpen.
+
+Section TypeOfFunc.
+  Context {typ func : Type}.
+  Context {RType_typ : RType typ}.
+  Context {RTypeOk_typ : RTypeOk}.
+  Context {RSym_func : RSym func}.
+    Lemma typeof_funcAs f t e (H : funcAs f t = Some e) : typeof_sym f = Some t.
+    Proof.
+      unfold funcAs in H.
+      generalize dependent (symD f).
+      destruct (typeof_sym f); intros; [|congruence].
+      destruct (type_cast t0 t); [|congruence].
+      destruct r; reflexivity.
+    Qed.
+    
+      Lemma funcAs_Some f t (pf : typeof_sym f = Some t) :
+        funcAs f t =
+        Some (match pf in (_ = z)
+          return match z with
+                   | Some z' => typD z'
+                   | None => unit
+                 end
+          with
+          | eq_refl => symD f
+          end).
+      Proof.
+        unfold funcAs.
+        generalize (symD f).
+        rewrite pf. intros.
+        rewrite type_cast_refl. reflexivity. apply _.
+      Qed.
+
+End TypeOfFunc.
+
+Section MakeOpenSound.
+  Context {typ func subst : Type} {ST : SubstType typ} {BT : BaseType typ} {RType_typ : RType typ}.
+  Context {OF : OpenFunc typ func} {ILF : ILogicFunc typ func} {BILF : BILogicFunc typ func} {BF : BaseFunc typ func}.
+  Context {LT : ListType typ}.
+  Context {EF : EmbedFunc typ func}.
+  Context {RelDec_string : RelDec (@eq (typD tyString))}.
+  Context {RelDec_typ : RelDec (@eq typ)}.
+  Context {RTypeOk_typ : RTypeOk}.
+  Context {RSym_func : RSym func}.
+  Context {RSym_funcOk : RSymOk RSym_func}.
+  Context {Typ2_tyArr : Typ2 _ Fun}.
+  Context {Typ0_Prop : Typ0 _ Prop}.
+  Context {Typ2_tyArrOk : Typ2Ok Typ2_tyArr}.
+  Context {HV : ValNull (typD tyVal)}.
+  Context {HSTD : SubstTypeD}.
+  Context {HBTD : BaseTypeD} {HLTD : ListTypeD}.
+  Context {OFOK : OpenFuncOk typ func}.
+
+  Let tyArr : typ -> typ -> typ := @typ2 _ _ _ _.
+
+  Let Expr_expr := Expr_expr (typ := typ) (func := func).
+  Let ExprOk_expr := ExprOk_expr (typ := typ) (func := func).
+  Let ExprUVar_expr := ExprUVar_expr (typ := typ) (func := func).
+  
+  Local Existing Instance Expr_expr.
+  Local Existing Instance ExprOk_expr.
+  Local Existing Instance ExprUVar_expr.
+
+  Local Notation "'tyStack'" := (tyArr tyString tyVal).
+
+  Lemma mkNull_sound (tus tvs : tenv typ) (f : func)
+    (df : typD tyVal)
+    (Ho : open_funcS f = Some of_null)
+    (Hf : funcAs f tyVal = Some df) :
+    exprD' tus tvs tyVal mkNull = Some (fun _ _ => df).
+  Proof.
+    unfold mkNull; simpl.
+    autorewrite with exprD_rw; simpl; forward; inv_all; subst.
+    pose proof (of_funcAsOk _ Ho) as H; rewrite H in Hf.
+    pose proof (of_fNullOk) as H1.
+    pose proof (of_funcAsOk _ H1) as H2. rewrite <- H2 in Hf.
+    pose proof (OpenFunc_typeOk _ H1) as H3. simpl in H3.
+    rewrite (funcAs_Some _ H3).
+    rewrite (funcAs_Some _ H3) in Hf.
+    inv_all; subst. reflexivity.
+  Qed.
+
+  Lemma mkApplySubst_sound (tus tvs : tenv typ) (t : typ) (f : func) (e s : expr typ func)
+    (df : typD (tyArr (tyArr tyStack t) (tyArr tySubst (tyArr tyStack t))))
+    (de : ExprI.exprT tus tvs (typD (tyArr tyStack t)))
+    (ds : ExprI.exprT tus tvs (typD tySubst))
+    (Ho : open_funcS f = Some (of_apply_subst t))
+    (Hf : funcAs f
+            (tyArr (tyArr tyStack t)
+              (tyArr tySubst (tyArr tyStack t))) = Some df)
+    (Hs : exprD' tus tvs tySubst s = Some ds)
+    (He : exprD' tus tvs (tyArr tyStack t) e = Some de) : 
+    exprD' tus tvs (tyArr tyStack t) (mkApplySubst t e s) =
+      Some (exprT_App (exprT_App (fun _ _ => df) de) ds).
+  Proof.
+    unfold mkApplySubst; simpl.
+    pose proof (exprD_typeof_Some _ _ _ _ _ Hs) as Hts.
+    pose proof (exprD_typeof_Some _ _ _ _ _ He) as Hte.
+    autorewrite with exprD_rw; simpl; forward; inv_all; subst.
+    autorewrite with exprD_rw; simpl; forward; inv_all; subst.
+    autorewrite with exprD_rw; simpl; forward; inv_all; subst.
+    pose proof (of_funcAsOk _ Ho) as H3; rewrite H3 in Hf.
+    pose proof (of_fApplySubstOk t) as H5.
+    pose proof (of_funcAsOk _ H5) as H6. rewrite <- H6 in Hf.
+    pose proof (OpenFunc_typeOk _ H5) as H7. simpl in H7.
+    unfold tyArr in *.
+    rewrite (funcAs_Some _ H7).
+    rewrite (funcAs_Some _ H7) in Hf.
+    inv_all; subst. reflexivity.
+  Qed.
+
+End MakeOpenSound.
