Charge!/src/Charge/Tactics/PullQuant/EmbedPullQuant.v
@@ -1,0 +1,45 @@
+Require Import MirrorCore.Lambda.ExprCore.
+Require Import MirrorCore.Lambda.Red.
+Require Import MirrorCore.Lambda.ExprLift.
+Require Import MirrorCore.TypesI.
+
+Require Import ExtLib.Core.RelDec.
+
+Require Import Charge.SetoidRewrite.Base.
+Require Import Charge.SetoidRewrite.AutoSetoidRewrite.
+Require Import Charge.ModularFunc.ILogicFunc.
+Require Import Charge.ModularFunc.EmbedFunc.
+
+Require Import Charge.Logics.ILogic.
+
+Section EILPullQuant.
+  Context {typ func : Type} {HIL : ILogicFunc typ func} {HB : EmbedFunc typ func}.
+  Context {RType_typ : RType typ}.
+  Context {RelDec_func : RelDec (@eq (expr typ func))}.
+
+  Let Rbase := expr typ func.
+
+  Variable rg_eq : typ -> expr typ func.
+
+  Definition rw_under_exists (t : typ) (l : typ) (rw : rewriter _) :=
+    rw_under (RGinj (rg_eq t))
+             (fun e rvars rg => rg_fmap (mkExists t l) (rw e rvars rg)).
+
+  Definition eil_match_plus (rw : rewriter _) (e : expr typ func) (rvars : list (RG (expr typ func))) (rg : RG Rbase) : m (expr typ func) :=
+    match e with
+      | App a (App b (Abs _ P)) =>
+        match embedS (typ := typ) (func := expr typ func) a, ilogicS b with 
+      	  | Some (eilf_embed u v), Some (ilf_exists t l) =>
+	    rg_plus
+	      (rg_bind (unifyRG (@rel_dec (expr typ func) _ _) rg (RGflip (RGinj (fEntails v))))
+	               (fun _ => rw_under_exists t v rw (mkEmbed u v P) rvars rg))
+	      (rg_bind (unifyRG (@rel_dec (expr typ func) _ _) rg (RGinj (fEntails v)))
+	               (fun _ => rw_under_exists t v rw (mkEmbed u v P) rvars rg))
+	  | _, _ => rg_fail
+	end
+      | _ => rg_fail
+    end.
+
+End EILPullQuant.
+
+Implicit Arguments eil_match_plus [[typ] [func] [HIL] [HB] [RelDec_func]].
