Charge!/src/Charge/Tactics/Rtac/Cancellation.v
@@ -1,0 +1,187 @@
+Require Import ExtLib.Core.RelDec.
+
+Require Import MirrorCore.Lambda.Expr.
+Require Import MirrorCore.RTac.RTac.
+Require Import MirrorCore.Lambda.ExprSubst.
+Require Import MirrorCore.Lambda.ExprUnify_simul.
+Require Import MirrorCore.Lambda.ExprVariables.
+Require MirrorCore.syms.SymEnv.
+Require MirrorCore.syms.SymSum.
+Require Import MirrorCore.VariablesI.
+
+Require Import Charge.Tactics.OrderedCanceller.
+Require Import Charge.Tactics.BILNormalize.
+Require Import Charge.Tactics.SynSepLog.
+Require Import Charge.Tactics.SepLogFoldWithAnd.
+Require Import Charge.ModularFunc.ILogicFunc.
+Require Import Charge.ModularFunc.BILogicFunc.
+
+Set Implicit Arguments.
+Set Strict Implicit.
+
+Section Canceller.
+  Context (typ func subst : Type) (tyLogic : typ).
+  Context {HIL : ILogicFunc typ func} {HBIL : BILogicFunc typ func}.
+  Context {RType_typ : RType typ} {RelDec_typ : RelDec (@eq typ)}.
+  Context {Typ2_typ : Typ2 RType_typ Fun}.
+  Context {RSym_func : @RSym _ RType_typ func}.
+  Existing Instance Expr_expr.
+  Context {SS : Subst subst (expr typ func)}.
+  Context {SU : SubstUpdate subst (expr typ func)}.
+  Context {SO : SubstOk SS}.
+  Context {MA : MentionsAny (expr typ func)}.
+  Context {uis_pure : expr typ func -> bool}.
+
+  Definition sls : SepLogAndSpec typ func :=
+  {| is_pure := fun e : expr typ func =>
+                  match ilogicS e with
+		    | Some (ilf_true _)
+		    | Some (ilf_false _) => true
+		    | _ => uis_pure e
+		  end
+   ; is_emp := fun e => false
+   ; is_star := fun e : expr typ func =>
+ 		  match bilogicS e with
+ 		    | Some (bilf_star _) => true
+ 		    | _ => false
+ 		  end
+   ; is_and := fun e : expr typ func =>
+ 		  match ilogicS e with
+ 		    | Some (ilf_and _) => true
+ 		    | _ => false
+ 		  end
+   |}.
+
+  Let doUnifySepLog c (tus tvs : EnvI.tenv typ) (s : ctx_subst (typ := typ) (expr := expr typ func) c) (e1 e2 : expr typ func)
+  : option (ctx_subst c) :=
+    @exprUnify (ctx_subst c) typ func RType_typ RSym_func Typ2_typ _ _ 10 tus tvs 0 e1 e2 tyLogic s.
+
+  Let ssl : SynSepLog typ func :=
+  {| e_star := fun l r =>
+                 match bilogicS l with
+                   | Some (bilf_emp _) => r
+                   | _ => match bilogicS r with
+                            | Some (bilf_emp _) => l
+                            | _ => mkStar tyLogic l r
+                          end
+                 end
+   ; e_emp := mkEmp tyLogic
+   ; e_and := fun l r =>
+                match ilogicS l with
+                  | Some (ilf_true _) => r
+                  | _ => match ilogicS r with
+                           | Some (ilf_true _) => l
+                           | _ => mkAnd tyLogic l r
+                         end
+                end
+   ; e_true := mkTrue tyLogic
+   |}.
+
+  Definition eproveTrue c (s : ctx_subst (typ := typ) (expr := expr typ func) c) (e : expr typ func) : option (ctx_subst c) :=
+    match ilogicS e with
+      | Some (ilf_true _) => Some s
+      | _ => None
+    end.
+
+  Definition is_solved (e1 e2 : conjunctives typ func) : bool :=
+    match e1 , e2 with
+      | {| spatial := e1s ; star_true := t ; pure := _ |}
+        , {| spatial := nil ; star_true := t' ; pure := nil |} =>
+        if t' then
+          (** ... |- true **)
+          true
+        else
+          (** ... |- emp **)
+          if t then false else match e1s with
+                                 | nil => true
+                                 | _ => false
+                               end
+      | _ , _ => false
+    end.
+Check @OrderedCanceller.ordered_cancel.
+
+  Definition the_canceller tus tvs (lhs rhs : expr typ func) c
+             (s : ctx_subst c)
+  : (expr typ func * expr typ func * (ctx_subst c)) + (ctx_subst c) :=
+    match @normalize_and typ _ _ func _ ssl sls tus tvs tyLogic lhs
+        , @normalize_and typ _ _ func _ ssl sls tus tvs tyLogic rhs
+    with
+      | Some lhs_norm , Some rhs_norm =>
+        match lhs_norm tt , rhs_norm tt with
+          | Some lhs_norm , Some rhs_norm =>
+            let '(lhs',rhs',s') :=
+                OrderedCanceller.ordered_cancel (subst := ctx_subst c)
+                  (doUnifySepLog (c := c) tus tvs) (eproveTrue (c := c))
+                  ssl
+                  (simple_order (func:=func)) lhs_norm rhs_norm s
+            in
+            if is_solved lhs' rhs' then
+              inr s'
+            else
+              inl (conjunctives_to_expr ssl lhs',
+                   conjunctives_to_expr ssl rhs',
+                   s')
+          | _ , _ => inl (lhs, rhs, s)
+        end
+      | _ , _ => inl (lhs, rhs, s)
+    end.
+
+  Let tyArr : typ -> typ -> typ := @typ2 _ _ _ _.
+
+  Definition CANCELLATION : rtac typ (expr typ func) :=
+    fun tus tvs nus nvs c s e =>
+      match e with
+        | App (App f L) R =>
+          match ilogicS f with
+	    | Some (ilf_entails t) =>
+	      match t ?[ eq ] tyLogic with
+	     	| true =>
+		  match the_canceller tus tvs L R s with
+		    | inl (l,r,s') =>
+		      match bilogicS r with (* This is for intuitionistic logics only *)
+		        | Some (bilf_emp _) => Solved s'
+		        | _ => let e' := mkEntails tyLogic l r in
+			       More s (GGoal e')
+		      end
+		    | inr s' => Solved s'
+		  end
+		| false => More s (GGoal e)
+	      end
+	    | _ => More s (GGoal e)
+	  end
+        | _ => More s (GGoal e)
+      end.  
+      
+      
+Definition the_canceller2 tus tvs (lhs rhs : expr typ func) :=
+    match @normalize_and typ _ _ func _ ssl sls tus tvs tyLogic lhs
+        , @normalize_and typ _ _ func _ ssl sls tus tvs tyLogic rhs
+    with
+      | Some lhs_norm , Some rhs_norm =>
+        match lhs_norm tt , rhs_norm tt with
+          | Some lhs_norm , Some rhs_norm =>
+            Some (simple_order (func := func) lhs_norm,
+                  simple_order (func := func) rhs_norm)
+          | _ , _ => None
+        end
+      | _ , _ => None
+    end.
+
+  Definition CANCELLATION2 tus tvs e :=
+      match e with
+        | App (App f L) R =>
+          match ilogicS f with
+	    | Some (ilf_entails t) =>
+	      match t ?[ eq ] tyLogic with
+	     	| true => the_canceller2 tus tvs L R
+		    | false => None
+	      end
+	    | _ => None
+	  end
+        | _ => None
+      end.
+
+End Canceller.
+
+Implicit Arguments CANCELLATION [[HIL] [HBIL] [RType_typ] [RelDec_typ]
+                                [Typ2_typ] [RSym_func] [MA]].
