Charge!/src/Charge/Tactics/Rtac/Instantiate.v
@@ -1,0 +1,14 @@
+Require Import MirrorCore.RTac.RTac.
+Require Import MirrorCore.Lambda.Expr.
+Require Import MirrorCore.Lambda.ExprSubst.
+
+Section InstantiateTac.
+	Context {typ func : Type}.
+	Context {EU : ExprUVar (expr typ func)}.
+
+	Definition INSTANTIATE := 
+		@INSTANTIATE typ (expr typ func) EU.
+
+End InstantiateTac.
+
+Implicit Arguments INSTANTIATE [[EU]].
