Charge!/src/Charge/Tactics/Rtac/Subst.v
@@ -1,0 +1,858 @@
+Require Import String.
+Require Import ExtLib.Core.RelDec.
+Require Import ExtLib.Tactics.
+Require Import MirrorCore.Lambda.Expr.
+Require Import MirrorCore.Lambda.ExprVariables.
+Require Import MirrorCore.Lambda.AppN.
+Require Import MirrorCore.TypesI.
+Require Import MirrorCore.RTac.RTac.
+Require Import MirrorCore.Lambda.RedAll.
+
+Require Import Charge.ModularFunc.BaseFunc.
+Require Import Charge.ModularFunc.OpenFunc.
+Require Import Charge.ModularFunc.ILogicFunc.
+Require Import Charge.ModularFunc.BILogicFunc.
+Require Import Charge.ModularFunc.LaterFunc.
+Require Import Charge.ModularFunc.EmbedFunc.
+Require Import Charge.ModularFunc.ListFunc.
+Require Import Charge.ModularFunc.SubstType.
+Require Import Charge.ModularFunc.BaseType.
+Require Import Charge.ModularFunc.ListType.
+Require Import Charge.Open.Stack.
+
+Set Implicit Arguments.
+Set Strict Implicit.
+
+Section ApplySubst.
+	Context {typ func : Type} {RType_typ : RType typ} {ST : SubstType typ} {BT : BaseType typ}
+	        {HOF : OpenFunc typ func} {HLF : ListFunc typ func} {HBF : BaseFunc typ func}.
+	Context {RelDec_typ : RelDec (@eq typ)}.
+	Context {RelDec_string : RelDec (@eq (typD tyString))}.
+
+    Variable Typ2_tyArr : Typ2 _ Fun.
+    Let tyArr : typ -> typ -> typ := @typ2 _ _ _ _.
+
+	Definition applySingleSubst (p : expr typ func) (x y : String.string) e :=
+		if x ?[ eq ] y then e else p.
+		    	
+    Fixpoint applyParSubst (p : expr typ func) (x : String.string) vs es :=
+    	match es with
+    		| App (App f e) es =>
+    			match vs, listS f with
+    				| v :: vs, Some (pCons t) =>
+    					if t ?[ eq ] tyArr tyString tyVal then
+    						if x ?[ eq ] v then
+    							e
+    						else
+    							applyParSubst p x vs es
+    					else
+    						p
+    				| _, _ => p
+    			end
+    		| _ => p
+    	end.
+    						
+    Fixpoint applyTruncSubst (p : expr typ func) (x : String.string) vs es :=
+    	match es with
+    		| App (App f e) es =>
+    			match vs, listS f with
+    				| v :: vs, Some (pCons t) =>
+    					if t ?[ eq ] tyArr tyString tyVal then
+    						if x ?[ eq ] v then
+    							e
+    						else
+    							applyParSubst p x vs es
+    					else
+    						fNull
+    				| _, _ => fNull
+    			end
+    		| _ => fNull
+    	end.				
+Check @open_funcS.
+Print baseS.
+	Definition applySubst (t : typ) (f e : expr typ func) (x : String.string) :=
+		match f with
+		  | App (App g e') y =>
+		  	match open_funcS g, baseS y with
+		  	  | Some (of_singleSubst), Some (pString v) => applySingleSubst e x v e'
+		  	  | _, _ => mkApplySubst t e f
+		  	end
+		  | _ => mkApplySubst t e f
+(*		  | mkApplySubst [t, p, mkSubstList [mkVarList [vs], es]] => applyParSubst p x vs es
+		  | mkApplyTruncSubst [t, p, mkSubstList [mkVarList [vs], es]] => applyTruncSubst x vs es*)
+		end.
+
+End ApplySubst.
+
+Section PushSubst.
+  Context {typ func : Type} {ST : SubstType typ} {BT : BaseType typ} {RType_typ : RType typ}.
+  Context {OF : OpenFunc typ func} {ILF : ILogicFunc typ func} {BILF : BILogicFunc typ func} {HBF : BaseFunc typ func}.
+  Context {EF : EmbedFunc typ func}.
+  Context {RelDec_string : RelDec (@eq (typD tyString))}.
+  Context {RelDec_type : RelDec (@eq typ)}.
+  
+  Variable Typ2_tyArr : Typ2 _ Fun.
+  Let tyArr : typ -> typ -> typ := @typ2 _ _ _ _.
+
+  Variable f : expr typ func.
+
+
+  Fixpoint pushSubst (e : expr typ func) (t : typ) : expr typ func :=
+    match e with
+    	| App (App g p) q =>
+    		match ilogicS g with
+    			| Some (ilf_and l) => mkAnd l (pushSubst p l) (pushSubst q l)
+    			| Some (ilf_or l) => mkOr l (pushSubst p l) (pushSubst q l)
+    			| Some (ilf_impl l) => mkImpl l (pushSubst p l) (pushSubst q l)
+    			| _ => match open_funcS g with
+		    			 | Some (of_ap t1 t2) => mkAp t1 t2 (pushSubst p (tyArr t1 t2))
+		    			             									 (pushSubst q t2)
+		    			 | _ => match bilogicS g with
+		    			          | Some (bilf_star l) => mkStar l (pushSubst p l) (pushSubst q l)
+		    			          | Some (bilf_wand l) => mkWand l (pushSubst p l) (pushSubst q l)
+		    			 	      | _ => mkApplySubst t e f
+		    			 	    end
+		    		   end
+    		end
+    	| App g p =>
+    		match open_funcS g, baseS p with
+    			| Some of_stack_get, Some (pString x) => applySubst t f e x
+    			| Some (of_const _), _ => e
+    			| _, _ => match embedS g with
+    					    | Some (eilf_embed u v) => mkEmbed u v (pushSubst p u)
+    					    | _ => mkApplySubst t e f
+    					  end
+    		end
+    	| _ => match ilogicS e with
+    		     | Some (ilf_true l) => mkTrue l
+    		     | Some (ilf_false l) => mkFalse l
+    		     | _ => match bilogicS e with
+    		     		  | Some (bilf_emp l) => mkEmp l
+    		     		  | _ => mkApplySubst t e f
+    		     		end
+    		   end
+    end.
+    
+End PushSubst.
+(*
+Implicit Arguments typeof_funcAs [[typ] [func] [RType_typ] [RSym_func] [f] [t] [e]].
+*)
+
+Section SubstTac.
+  Context {typ func subst : Type} {ST : SubstType typ} {BT : BaseType typ} {RType_typ : RType typ}.
+  Context {OF : OpenFunc typ func} {ILF : ILogicFunc typ func} {BILF : BILogicFunc typ func} {BF : BaseFunc typ func}.
+  Context {LT : ListType typ}.
+  Context {EF : EmbedFunc typ func}.
+  Context {RelDec_string : RelDec (@eq (typD tyString))}.
+  Context {RelDec_typ : RelDec (@eq typ)}.
+  Context {RTypeOk_typ : RTypeOk}.
+  Context {RSym_func : RSym func}.
+  Context {RSym_funcOk : RSymOk RSym_func}.
+  Variable Typ2_tyArr : Typ2 _ Fun.
+  Variable Typ0_Prop : Typ0 _ Prop.
+  Context {Typ2_tyArrOk : Typ2Ok Typ2_tyArr}.
+  Context {HV : ValNull (typD tyVal)}.
+  Context {HSTD : SubstTypeD}.
+  Context {HBTD : BaseTypeD} {HLTD : ListTypeD}.
+  Context {OFOK : OpenFuncOk typ func}.
+  Context {gs : @logic_ops _ RType_typ}.
+  Context {bs : @bilogic_ops _ RType_typ}.
+  Context {ILFOK : ILogicFuncOk typ func gs}.
+  Context {BILFOK : BILogicFuncOk typ func bs}.
+  Let tyArr : typ -> typ -> typ := @typ2 _ _ _ _.
+
+  Let Expr_expr := Expr_expr (typ := typ) (func := func).
+  Let ExprOk_expr := ExprOk_expr (typ := typ) (func := func).
+  Let ExprUVar_expr := ExprUVar_expr (typ := typ) (func := func).
+  
+  Local Existing Instance Expr_expr.
+  Local Existing Instance ExprOk_expr.
+  Local Existing Instance ExprUVar_expr.
+
+  Definition substTac (_ : list (option (expr typ func))) (e : expr typ func) (args : list (expr typ func))
+  : expr typ func :=
+    match open_funcS e with
+	  | Some (of_apply_subst t) =>
+	    match args with
+	      | e :: f :: nil =>
+	        pushSubst Typ2_tyArr f e t
+	      | _ => apps e args
+	    end
+	  | _ => apps e args
+	end.
+Require Import Charge.Open.Subst.	
+Require Import MirrorCore.Lambda.ExprTac.
+Require Import FunctionalExtensionality.	
+  
+      Lemma Rcast_eq_refl (t : typ) (F : Type -> Type) (a b : F (typD t)) (H : Rcast F eq_refl a = b) : a = b.
+      Proof.
+        apply H.
+      Qed.
+
+    Lemma exprT_App_wrap tus tvs (t u : typ) (f : HList.hlist typD tus -> HList.hlist typD tvs -> typD t -> typD u) (a : exprT tus tvs (typD t)) :
+      exprT_App (fun us vs => fun1_wrap _ (f us vs)) a = fun us vs => (f us vs) (a us vs).
+    Proof.
+      unfold fun1_wrap, exprT_App, eq_rect_r, eq_sym, eq_rect.
+      forward.
+    Qed.
+
+  Lemma substTac_ok : partial_reducer_ok (substTac nil).
+  Proof.
+    admit.
+  Qed.
+    (*
+    unfold partial_reducer_ok; intros.
+    unfold substTac; simpl.
+    destruct e; try (exists val; tauto).
+    remember (open_funcS f). destruct o; try (exists val; tauto).
+    destruct o; try (exists val; tauto).
+    destruct es; try (exists val; tauto).
+    destruct es; try (exists val; tauto).
+    destruct es; try (exists val; tauto).
+    simpl in H.
+    autorewrite with exprD_rw in H; simpl in H; forward; inv_all; subst.
+    autorewrite with exprD_rw in H0; simpl in H0; forward; inv_all; subst.
+    autorewrite with exprD_rw in H2; simpl in H2; forward; inv_all; subst.
+    
+    symmetry in Heqo.
+    pose proof (typeof_funcAs _ _ H2).
+    pose proof (OpenFunc_typeOk _ Heqo).
+    rewrite H4 in H5. simpl in H5.
+    inversion H5; subst.
+    apply typ2_inj in H7 as [H7 H8]; [|apply _].
+    apply typ2_inj in H8 as [H8 H9]; [|apply _].
+    unfold Rty in *.
+    subst; inv_all; subst.
+    clear H6 H12 H11 H5 H8 H10 H9 H4.
+    induction e using expr_strong_ind;
+    try (solve [simpl; eexists; split; [eapply mkApplySubst_sound; eassumption|reflexivity]]).
+    + (* True, False, and Emp *)
+      autorewrite with exprD_rw in H3; simpl in H3; forward; inv_all; subst.
+	  simpl; remember (ilogicS i) as o; destruct o; [destruct i0|];
+	  try (remember (bilogicS i) as o; destruct o; [destruct b|]);
+	  try (solve [simpl; eexists; split; [eapply mkApplySubst_sound; try eassumption; autorewrite with exprD_rw; simpl; forward; inv_all; subst; reflexivity|reflexivity]]).
+	  autorewrite with exprD_rw in H0; simpl in *.
+
+      pose proof (of_funcAsOk).
+      specialize (H4 _ _ Heqo).
+      rewrite H4 in H2.
+      unfold funcAs in H2. simpl in H2. rewrite type_cast_refl in H2. unfold Rrefl in H2.
+      apply Rcast_eq_refl in H2. inversion H2; subst; clear H2.
+      unfold fun3_wrap.
+      unfold fun2_wrap.
+      rewrite exprT_App_wrap.
+      rewrite exprT_App_wrap.
+      symmetry in Heqo1.
+      eexists. split.
+      eapply mkEmp_sound; [eapply Heqo1|eapply H3].
+      intros.
+      pose proof (bilf_funcAsOk i Heqo1). simpl in H4.
+      rewrite H2 in H3.
+      unfold funcAs in H3; simpl in H3; forward.
+      unfold Rty in r.
+      subst.
+      apply Rcast_eq_refl in H6. inv_all; subst.
+      Check fun1D.
+      unfold fun1_wrap, fun1D, eq_rect_r, eq_rect, eq_sym.
+      remember (typ2_cast (typ2 tyString tyVal) t0).
+      inversion e; subst.
+      remember (typ2_cast (typ2 tyString tyVal) t0).
+      generalize dependent e.
+      rewrite H7.
+      rewrite H7 in e.
+      do 2 rewrite typ2_cast in H7.
+      unfold Fun in H7.
+      remember (typ2_cast (typ2 tyString tyVal) t0).
+      rewrite (UIP_refl H7).
+      assert (forall (x:Type) (p:x = x), p = eq_refl x) by admit.
+      remember (typ2_cast (typ2 tyString tyVal) t0).
+      unfold Fun in e.
+      subst.
+      remember (typ2_cast (typ2 tyString tyVal) t0).
+      unfold id.
+      remember (typ2_cast tyString tyVal).
+      assert(forall (x y:Type) (p1 p2:x = y), p1 = p2) by admit.
+      pose proof e1 as e3.
+      specialize (H7 _ _ e1 e3).
+      assert (typD (typ2 tyString tyVal) = Fun (typD tyString) (typD tyVal)) by (apply typ2_cast).
+      generalize dependent e3.
+      rewrite H8.
+      subst.
+      Check typ2_cast.
+      rewrite (@typ2_cast typ RType_typ Fun _ tyString tyVal).
+      generalize dependent (fun y : typD (typ2 tyString tyVal) =>
+    apply_subst
+      (fun x : stack (typD tyString) (typD tyVal) =>
+       match e in (_ = y0) return (id y0) with
+       | eq_refl => BILogic.empSP
+       end
+         match
+           match
+             typ2_cast tyString tyVal in (_ = y0)
+             return (y0 = typD (typ2 tyString tyVal))
+           with
+           | eq_refl => eq_refl
+           end in (_ = y0) return (id y0)
+         with
+         | eq_refl => x
+         end)
+      match stSubst in (_ = y0) return (id y0) with
+      | eq_refl => e2 us vs
+      end).
+      
+      
+      assert (typD (typ2 (typ2 tyString tyVal) t0) = Fun (typD (typ2 tyString tyVal)) (typD t0)) by (apply typ2_cast).
+      progress eapply eq_ind_r with (typD (typ2 (typ2 tyString tyVal) t0)); [|symmetry; eapply H7].
+      subst.
+      assert (typD (typ2 tyString tyVal) = Fun (typD tyString) (typD tyVal)) by (apply typ2_cast).
+      subst.
+      apply typ2_cast.
+      SearchAbout typD typ2.
+      generalize dependent e.
+      Check typ2_cast.
+      
+      rewrite (@typ2_cast typ RType_typ Fun _ tyString tyVal).
+ specialize (H6 _ Heqe).
+      SearchAbout typ2_cast.
+      Check typ2_cast.
+      generalize dependent (e2 us vs). intros.
+      generalize dependent (BILogic.empSP). intros.
+      generalize dependent (typ2_cast tyString tyVal). intros.
+      generalize dependent (typ2_cast (typ2 tyString tyVal)).
+      intros.
+      destruct stSubst.
+      destruct e.
+      destruct e.
+      destruct (typ2_cast tyString tyVal).
+      
+      destruct (typ2_cast (typ2 tyString tyVal) t0).
+      Lemma blurb f : (fun x => (fun1D Typ2_tyArr f) (fun1_wrap Typ2_tyArr x)) = fun1D _ f.
+      
+      unfold fun1_wrap.
+      unfold eq_rect_r, eq_rect, eq_sym. simpl. forward.
+      specialize (H5 (typ2 (typ2 tyString tyVal) t0)).
+      rewrite H5 in H3. simpl. inv_all; subst. simpl in H3.
+      Check bilf_funcAsOk.
+      simpl in H3.
+      unfold funcAs in H3. simpl in H3. forward. inv_all; subst.
+     destruct r; subst. 
+     
+     
+      Lemma Rcast_option (t u : typ) (r : Rty t u) (a : typD t) (b : typD u) (H : Rcast option r (Some a) = Some b) :
+        Rcast (fun T => T) r a = b.
+      Proof.
+        unfold Rcast, Relim, Rsym in *.
+        destruct r; unfold eq_sym in *.
+        inversion H; subst; reflexivity.
+      Qed.
+      
+      apply Rcast_eq_refl in H7.
+      inversion H7; subst; clear H7.
+      
+      
+      
+      apply Rcast_option in H7.
+      unfold Rcast, Relim, Rsym, eq_sym in H7.
+      destruct r. subst.
+      simpl in *.
+      SearchAbout Rcast.
+      Check Rcast.
+      Print Rcast.
+      unfold Rcast, Relim, Rsym, eq_sym in H7.
+      forward.
+      unfold Rty in r.
+      SearchAbout type_cast.
+      unfold type_cast in H6. simpl in H6.
+      rewrite r in H7.
+      pose proof (bilf_fStarOk logic0) as HfuncOk.
+      rewrite H4 in *.
+      specialize
+      Lemma test tus tvs (t u : typ) (f : exprT tus tvs (typD (typ2 t u))) g us vs : exists x, exprT_App f g us vs = x.
+      Proof.
+        unfold exprT_App.
+        simpl.
+        unfold eq_sym.
+        generalize dependent ( fun (f0 : exprT tus tvs (typD t -> typD u))
+        (x0 : exprT tus tvs (typD t)) (us0 : HList.hlist typD tus)
+        (vs0 : HList.hlist typD tvs) => f0 us0 vs0 (x0 us0 vs0)). intros.
+        SearchAbout typ2_cast.
+        unfold typ2_cast. simpl.
+        destruct (typ2_cast t u).
+      unfold exprT_App.
+      simpl.
+      SearchAbout exprT_App.
+      unfold exprT_App, eq_sym.
+      destruct (typ2_cast (typ2 (typ2 tyString tyVal) t0)
+         (typ2 tySubst (typ2 (typ2 tyString tyVal) t0))).
+      destruct (typ2_cast tySubst (typ2 (typ2 tyString tyVal) t0)).
+      unfold exprT_App.
+      simpl.
+      reflexivity.
+      unfold exprT_App. intros. simpl.
+      rewrite mkEmp_sound with (f := i).
+      setoid_rewrite mkEmp_sound.
+      eexists. split. erewrite mkEmp_sound.
+      erewrite mkEmp_sound.
+      Focus 3. eapply H3.
+      eexists. split.
+      eexists; split; [reflexivity|].
+      eexists.
+      split.
+      eapply mkEmp_sound; try eassumption.
+      rewrite mkEmp_sound.
+      Check mkEmp_sound.
+      eapply mkEmp_sound.
+      rewrite mkEmp_sound.
+      setoid_rewrite mkEmp_sound.
+      SearchAbout exprT_App.
+      unfold exprT_App. simpl.
+      eexists. split.
+      autorewrite with exprD_rw. simpl.
+      Print funcAs.
+      Print RType.
+      Print RSym.
+      Print funcAs.
+      unfold funcAs.
+      assert (typeof_sym (fEmp logic0) = Some logic0).  admit.
+      rewrite H4.
+      Print symD.
+      unfold symD. simpl.
+            Require Import Charge.Logics.BILogic.
+      SearchAbout typ2 typD.
+      Print Typ2_tyArr.
+      unfold exprT, OpenT. simpl.
+      rewrite (@typ2_cast typ RType_typ Fun Typ2_tyArr (typ2 tyString tyVal) t0).
+      unfold typ2. simpl. unfold exprT. simpl. unfold OpenT. simpl. unfold Ty
+      exists (fun _ _ => empSP).
+      
+      
+      try (solve [simpl; eexists; split; [eapply mkApplySubst_sound; eassumption|reflexivity]]).
+      Focus 2.
+      simpl; eexists; split; [|reflexivity].
+      Check @ilf_true_type_eq.
+      symmetry in Heqo0.
+      pose proof (ilf_true_type_eq (gs := gs) _ _ Heqo0 H3).
+      rewrite H4 in *; clear H4.
+      erewrite (mkTrue_sound (gs := gs)); [|eassumption|eassumption].
+      rewrite (ilf_funcAsOk _ Heqo0) in H3.
+      unfold funcAs in H3; simpl in H3. forward; inv_all; subst.
+      unfold Rcast, Relim, Rsym, eq_sym in H5. simpl in H5.
+      rewrite type_cast_refl in H4.
+      unfold Rrefl in H4; inv_all; subst.
+      inv_all; subst.
+      rewrite (of_funcAsOk _ Heqo) in H2.
+      pose proof (of_fApplySubstOk t0).
+      pose proof (OpenFunc_typeOk _ H4).
+      simpl in H5.
+      unfold funcAs in H2; simpl in H2.
+      rewrite type_cast_refl in H2.
+      inv_all; subst.
+      
+      (* Gregory: This should be true, but I don't quite know where to go from here. *)
+      
+      unfold exprT_App, fun3_wrap, fun2_wrap, fun1_wrap, fun1D, id, eq_rect_r, eq_rect. uip_all'.
+      
+      (* This gives me a bunch of equivalence proofs, and a lot of typing problems *)
+      
+      unfold Fun in *.
+      unfold exprT_App. simpl.
+      rewrite funcAs_Some with (pf := H5) in H2.
+      Check funcAs_Some.
+      Check OpenFunc_typeOk.
+      unfold funcAs in H2; simpl in H2; forward; inv_all; subst.
+      rewrite type_cast_refl in H2; inv_all; subst.
+      unfold Rcast, Rrefl in H4; simpl in H4; inv_all; subst.
+      unfold Rcast, Rrefl, Relim, Rsym, eq_sym, fun3_wrap, fun2_wrap, fun1_wrap, eq_rect, eq_rect_r, eq_rect, eq_sym, fun1D, eq_rect.
+      simpl.
+      unfold exprT_App, eq_sym.
+      forward.
+      simpl.
+      inv_all; subst.
+      clear H2 H4.
+      uip_all.
+      unfold Fun in e3.
+      subst.
+      uip_all.
+      unfold id.
+      generalize dependent (typD (typ2 tyString tyVal)).
+      destruct e1.
+      uip_all'.
+      destruct stSubst.
+      destruct ( typ2_cast (typ2 tyString tyVal) t0).
+      forward.
+      SearchAbout typ2_cast.
+      unfold typ2_cast in H2.
+      rewrite type_cast_refl in H2.
+      inversion H2; subst. f_equal.
+      unfold exprT_App, fun3_wrap, eq_sym. simpl.
+      apply functional_extensionality. intros.
+      apply functional_extensionality. intros.
+      Check of_funcAsOk.
+      rewrite mkTrue_sound.
+      assert (exprD' tus tvs
+      try (solve [simpl; eexists; split; [apply mkApplySubst_sound | reflexivity]; assumption]).
+    simpl.
+    assumption.
+    assumption.
+    + simpl. eexists; split; [|reflexivity].
+      apply mkApplySubst_sound; assumption.
+    + simpl; eexists; split; [|reflexivity].
+      apply mkApplySubst_sound; assumption.
+    + 
+      autorewrite with exprD_rw in H3; simpl in H3; forward; inv_all; subst.
+      unfold Rty in r. subst.
+      unfold mkApplySubst. simpl.
+      autorewrite with exprD_rw; simpl; forward; inv_all; subst.
+      autorewrite with exprD_rw; simpl; forward; inv_all; subst.
+      pose (nth_error_get_hlist_nth_Some _ H3).
+      destruct e as [? ?].
+      rewrite x.
+      autorewrite with exprD_rw; simpl; forward; inv_all; subst.
+      rewrite type_cast_refl.
+      unfold Rcast_val, Rrefl, Rcast, Relim, Rsym, eq_sym; simpl.
+      assert (open_funcS (fApplySubst t0) = Some (of_apply_subst t0)) by admit.
+      assert (typeof_sym (of_apply_subst t0) = Some (typ2 (typ2 (typ2 tyString tyVal) t0)
+                   (typ2 tySubst (typ2 (typ2 tyString tyVal) t0)))) by admit.
+      pose proof (funcAsOk _ H3); rewrite H7.
+      pose proof (funcAs_Some _ H6).
+      rewrite H8. simpl.
+      f_equal. f_equal. f_equal.
+      Require Import FunctionalExtensionality.
+      apply functional_extensionality. intros.
+      apply functional_extensionality. intros.
+      clear -H6.
+      revert H6.
+      generalize (symD (of_apply_subst t0)).
+      intros.
+      admit.
+      apply _.
+    + eexists; split; [|reflexivity].
+      
+      simpl.
+      Check symD.
+      Print typD.
+      Print RType.
+      Check exprT_App.
+      Print exprT.
+ 
+Check @exprT_App.
+
+    generalize dependent (
+       (typ2 (typ2 (typ2 tyString tyVal) t)
+          (typ2 tySubst (typ2 (typ2 tyString tyVal) t)))).
+    generalize dependent (typD t0).
+    destruct z.
+    generalize dependent (typeof_sym (of_apply_subst t)).
+    rewrite H2.
+    destruct H2.
+    f_e
+    rewrite H.
+      progress autorewrite with exprD_rw; simpl; forward; inv_all; subst.
+      autorewrite with exprD_rw; simpl; forward; inv_all; subst.
+      
+      pose (nth_error_get_hlist_nth_Some _ H3).
+      destruct e as [? ?].
+      rewrite x.
+      autorewrite with exprD_rw; simpl; forward; inv_all; subst.
+      rewrite type_cast_refl.
+      unfold Rcast_val, Rrefl, Rcast, Relim, Rsym, eq_sym; simpl.
+      assert (open_funcS (fApplySubst t0) = Some (of_apply_subst t0)) by admit.
+      assert (typeof_sym (of_apply_subst t0) = Some (typ2 (typ2 (typ2 tyString tyVal) t0)
+                   (typ2 tySubst (typ2 (typ2 tyString tyVal) t0)))) by admit.
+      pose proof (funcAsOk _ H3); rewrite H7.
+      pose proof (funcAs_Some _ H6).
+      rewrite H8. simpl.
+      f_equal. f_equal. f_equal.
+      Require Import FunctionalExtensionality.
+      apply functional_extensionality. intros.
+      apply functional_extensionality. intros.
+      clear -H6.
+      revert H6.
+      generalize (symD (of_apply_subst t0)).
+      intros.
+      admit.
+      apply _.    
+      generalize  (typ2 (typ2 (typ2 tyString tyVal) t0)
+            (typ2 tySubst (typ2 (typ2 tyString tyVal) t0))).
+      generalize dependent (Some (typ2 (typ2 (typ2 tyString tyVal) t0)
+          (typ2 tySubst (typ2 (typ2 tyString tyVal) t0)))); intros; subst; reflexivity.
+      generalize (symD (of_apply_subst t0)).
+      intros. 
+      generalize dependent H6.
+      generalize dependent (Some (typ2 (typ2 (typ2 tyString tyVal) t0)
+          (typ2 tySubst (typ2 (typ2 tyString tyVal) t0)))); intros; subst; reflexivity.
+      generalize dependent H6.
+      uip_all.
+      subst.
+      destruct H6.
+      generalize dependent H6. uip_all'.
+      assert (symD (fApplySubst t0) = symD (of_apply_subst t0)).
+      assert (typo
+        Print symAs_Some.
+      
+      pose proof (funcAsOk _ H3). rewrite H6.
+      SearchAbout exprD' symD.
+      SearchAbout symD.
+
+      
+      Check symD.
+      SearchAbout funcAs symD.
+      Check funcAs.
+      
+      Print exprT_App.
+      assert (funcAs (fApplySubst t0)
+        (typ2 (typ2 (typ2 tyString tyVal) t0)
+           (typ2 tySubst (typ2 (typ2 tyString tyVal) t0))) = symD (of_apply_subst t0)).
+      destruct o.
+      admit.
+      unfold funcAs in Heqo0.
+      simpl in Heqo0.
+      admit.
+      assert False.
+      rewrite H3 in Heqo0.
+      forward.
+      rewrite H3.
+      rewrite type_cast_refl.
+      assert (open_funcS (fApplySubst t0) = Some (of_apply_subst t0)).
+      admit.
+      pose (funcAsOk _ H3). 
+      Check typeof_funcAs.
+      
+      rewrite e; clear e.
+      pose proof (OpenFunc_typeOk _ H3).
+      simpl.
+      unfold fApplySubst. simpl.
+      unfold funcAs.
+      simpl.
+      Transparent symD.
+      simpl.
+      SearchAbout nth_error nth_error_get_hlist_nth.
+      unfold nth_error.
+      progress autorewrite with exprD_rw; simpl; forward; inv_all; subst.
+      simpl in H3.
+    Check expr_strong_ind.
+    Check (fun (_ : HList.hlist typD tus) (_ : HList.hlist typD tvs) =>
+         symD (of_apply_subst t0)).
+    Check (fun (_ : HList.hlist typD tus) (_ : HList.hlist typD tvs) =>
+         @apply_subst).
+    Transparent symD.
+    simpl.
+    unfold fun3_wrap, fun2_wrap, eq_rect_r, eq_rect, eq_sym. simpl.
+    rewrite (@typ2_cast typ _ Fun _).
+    rewrite typ2_cast.
+    SearchAbout exprT_App.
+    unfold eq_rect_r, eq_rect, eq_sym.
+    SearchAbout typ2_cast.
+    Check @typ2_cast.
+    remember (typ2_cast (typ2 (typ2 tyString tyVal) t0)
+               (typ2 tySubst (typ2 (typ2 tyString tyVal) t0))).
+    destruct e1.
+    unfold typ2_cast.
+    Transparent symD. 
+    simpl.
+    refine (exists val' : exprT tus tvs (typD (typ2 (typ2 tyString tyVal) t0)),
+  ExprDsimul.ExprDenote.exprD' tus tvs (typ2 (typ2 tyString tyVal) t0)
+    (pushSubst Typ2_tyArr e0 e t0) = Some val' /\
+  (forall (us : HList.hlist typD tus) (vs : HList.hlist typD tvs),
+   P us vs ->
+   exprT_App
+     (exprT_App
+        _ e4) e2 us vs = val' us vs)).
+    simpl.
+    erewrite typ2_cast.
+    generalize dependent t3.
+    Transparent symD.
+    rewrite typ2_cast.
+    Print symD.
+    simpl in H2.
+    Example test t0 : exists x, x = typD (typ2 (typ2 (typ2 tyString tyVal) t0)
+          (typ2 tySubst (typ2 (typ2 tyString tyVal) t0))).
+    Proof.
+      repeat rewrite typ2_cast.
+      unfold Fun.
+      repeat rewrite btString.
+      rewrite stVal.
+      vm_compute.
+      destruct RType_typ. simpl.
+      destruct Typ2_tyArr.
+      simpl.
+      destruct BT. simpl. destruct ST. simpl.
+      SearchAbout typ2.
+      repeat rewrite typ2_cast.
+      unfold Fun. simpl.
+      destruct BT.
+      rewrite btString.
+    unfold funcAs in H2; simpl in H2.
+    rewrite type_cast_refl in H2.
+    unfold Rcast, Relim, Rrefl in H2. simpl in H2.
+    unfold eq_rect_r, eq_rect, Fun, eq_sym, eq_rect_r, typ2_cast in H2; simpl in H2.
+    destruct Typ2_tyArr; simpl in H2.
+    SearchAbout typ2_cast.
+    Print Typ2Ok.
+    Print typ2_match.
+    rewrite typ2_match_Proper in H2.
+    progress unfold typ2_cast in H2.
+    Print Rcast.
+    inv_all; subst.
+    unfold exprT_App, eq_sym, typ2_cast, exprT, OpenT, typ2_cast; simpl.
+    
+    rewrite type_cast_refl in H2.
+    SearchAbout Typ2.
+    unfold Rcast, Rrefl, eq_rect_r, eq_sym, eq_rect, typ2_cast in H2; simpl in H2.
+    
+    unfold Rcast, Rrefl, eq_rect_r, eq_sym, typ2_cast, Fun, eq_rect in H2; simpl in H2.
+    destruct Typ2_tyArr. simpl in H2.
+    unfold typD in H2. simpl in H2.
+    destruct RType_typ; simpl in *.
+    forward.
+    inv_all; subst.
+    unfold exprT_App, eq_sym. simpl.
+    uip_all'.
+    uip_all'.
+    destruct e3.
+    uip_all'.
+    revert H2. uip_all.
+    unfold eq_rect in H2.
+    inv_all; subst.
+    vm_compute in H2.
+    subst.
+    rewrite H8 in *.
+    inversion H7.
+    rewrite H7 in H2.
+    simpl in H4.
+    unfold typ2 in H2. simpl in H2.
+    destruct Typ2_tyArr.
+    simpl.
+    unfold typ2 in H2.
+    unfold funcAs in H2. simpl in H2.
+    forward.
+    generalize dependent t3.
+    subst.
+    unfold Rty in r.
+    rewrite <- r.
+    unfold Rcast, Relim, Rsym, eq_sym, eq_rect_r, eq_rect, eq_sym, typ2_cast, Fun, typD in H2; simpl in H2.
+    destruct RType_typ; simpl in *.
+    
+     destruct r.
+    simpl in H4.
+    unfold type_cast in H2. simpl in H2.
+    destruct RType_typ.
+    destruct r.
+    rewrite OpenFunc_typeOk in .
+    pose proof (
+       
+    assert (typeof_sym f = typeof_open_func _ (of_apply_subst t0)) by admit.
+    Check symD.
+    Check exprD.
+    Print RSymOk.
+    Print exprD'.
+    Print Expr.
+    Print exprT.
+    Print OpenT.
+    assert (funcAs f (typeof_open_func _ (of_apply_subst t0)) = 
+       Some (fun _ _ => @apply_subst (typD tyString) (typD tyVal) (typD t0))).
+    assert (funcAs ).
+    simpl in H4.
+    pose proof (typeof_funcAs H2) as H5.
+    rewrite H5 in H4; clear H5; inv_all; subst.
+
+
+    eexists; split; [|intros; reflexivity].
+
+    induction e using expr_strong_ind.
+    + simpl.
+    SearchAbout exprT_App.
+    
+    unfold exprT_App. simpl.
+    unfold exprT, OpenT. simpl.
+    split.
+    Focus 2.
+    intros. reflexivity.
+    exists e2.
+    + simpl in H0.
+      unfold exprT_App. simpl.
+      unfold exprT. simpl. unfold OpenT. simpl.
+      SearchAbout typ2_cast.
+    generalize dependent t3.
+    generalize dependent t2.
+    generalize dependent t1.
+    generalize dependent t.
+    generalize dependent tus.
+    generalize dependent tvs.
+    generalize dependent e.
+    generalize dependent e0.
+    subst.
+    rewrite H4.
+    remember (typeof_sym f).
+    rewrite H4 in H2.
+    simpl in H4. 
+    Check @UIP_refl.
+    revert H2 Heqo.
+    uip_all.
+    generalize dependent t3.
+    generalize dependent t2. generalize dependent t1. generalize dependent t.
+    generalize dependent tus. generalize dependent tvs. generalize dependent e.
+    generalize dependent e0.
+    symmetry in H4. setoid_rewrite <- H4.
+     generalize dependent func.
+    setoid_rewrite H4.
+     rewrite H4.
+    red in H4.
+    rewrite (@UIP_refl (option typ) _ _ H4) in H2.
+    U
+    Check UIP_rewrite.
+    UIP_rewrite
+    rewrite H4 in H2.
+    simpl. unfold typ2. simpl. unfold typ2. simpl.
+    destruct f. simpl in Heqo.
+    unfold funcAs in H2. simpl in H2.
+    unfold exprT_App, OpenT; simpl. uip_all.
+    rewrite (UIP_refl e1).
+	simpl in H. red_exprD.
+	Locate idred.
+Check idred.
+*)
+Print full_reducer.
+  Definition SUBST := SIMPLIFY (typ := typ) (fun _ _ _ _ => beta_all substTac).
+(*
+  Lemma substTac_ok : full_reducer_ok substTac.
+  Proof.
+    unfold full_reducer_ok; intros.
+    SearchAbout exprT.
+    Print OpenT.
+    unfold exprT, OpenT in *.
+Check hlist_build.
+SearchAbout apps.
+Print apps_sem'.
+Print apply_sem'.
+Check apps_sound.
+    Print var_termsP.
+    unfold applys. simpl.
+  Lemma substTac_sound   
+    (He : exprD' tus tvs (fold_right (typ2 (F := Fun)) t targs) e = Some de) :
+    exists de', exprD' tus' tvs' t (substTac var_terms e es) = Some de'
+    SearchAbout 
+    unfold OpenT.
+  Qed.
+Check @SIMPLIFY_sound.
+  Lemma SUBST_sound : @rtac_sound typ (expr typ func) RType_typ _ Expr_expr _ SUBST.
+  Proof.
+    unfold SUBST.
+    apply SIMPLIFY_sound.
+    intros; simpl; forward.
+    unfold propD, exprD'_typ0 in H3. forward; inv_all; subst.
+    destruct (beta_all_sound substTac_ok _ _ e1 H3) as [v [H4 H5]].
+    unfold propD, exprD'_typ0; simpl.
+    forward; inv_all; subst.
+    SearchAbout typ0_cast.
+    uip_all.
+    Check Pure_pctxD.
+    eapply Pure_pctxD; eauto.
+    intros us0 vs0; autorewrite with eq_rw. intro; rewrite H5. tauto.
+    assumption.
+  Qed.
+*)
+  
+End SubstTac.
+Print SUBST.
+Implicit Arguments SUBST [[ST] [RType_typ] [OF] [ILF] [BILF] [EF] [BF] [Typ2_tyArr]].
