Charge!/src/Charge/Tactics/SynSepLog.v
@@ -1,0 +1,699 @@
+(** This file introduces a syntactic separation logic.
+ **)
+Require Import Coq.Classes.Morphisms.
+Require Import ExtLib.Tactics.
+Require Import BILogic ILogic Pure.
+Require Import MirrorCore.EnvI.
+Require Import MirrorCore.SymI.
+Require Import MirrorCore.TypesI.
+Require Import MirrorCore.ExprI.
+Require Import MirrorCore.Lambda.Expr.
+
+Require Import Charge.Tactics.SepLogFold.
+
+Set Implicit Arguments.
+Set Strict Implicit.
+
+Section syn_sep_log.
+  Variable typ : Type.
+  Variable RType_typ : RType typ.
+  Variable Typ2_Fun : Typ2 _ Fun.
+  Variable sym : Type.
+  Variable RSym_sym : RSym sym.
+
+  Variable SL : typ.
+
+  Variable SLS : SepLogSpec typ sym.
+  Variable ILO : ILogicOps (typD SL).
+  Variable BILO : BILOperators (typD SL).
+  Variable IL : @ILogic _ ILO.
+  Variable BIL : @BILogic _ ILO BILO.
+
+  (** TODO: This seems to be defined at the wrong level of abstraction
+   ** It is the only piece here that requires that I be in [Ext.expr] rather
+   ** than an arbitrary [expr].
+   **)
+  Variable slsok : SepLogSpecOk _ RSym_sym SL SLS ILO BILO.
+
+  Record SynSepLog : Type :=
+  { e_star : expr typ sym -> expr typ sym -> expr typ sym
+  ; e_and : expr typ sym -> expr typ sym -> expr typ sym
+  ; e_emp : expr typ sym
+  ; e_true : expr typ sym
+  }.
+
+  Variable SSL : SynSepLog.
+
+  Record SynSepLogOk : Type :=
+  { e_empOk : forall tus tvs,
+              exists val,
+                exprD' tus tvs SL SSL.(e_emp) = Some val /\
+                forall us vs, val us vs -|- empSP
+  ; e_trueOk : forall tus tvs,
+               exists val,
+                 exprD' tus tvs SL SSL.(e_true) = Some val /\
+                 forall us vs, val us vs -|- ltrue
+  ; e_starOk : forall tus tvs x y valx valy,
+                 exprD' tus tvs SL x = Some valx ->
+                 exprD' tus tvs SL y = Some valy ->
+                 exists val,
+                   exprD' tus tvs SL (SSL.(e_star) x y) = Some val /\
+                   forall us vs, val us vs -|- valx us vs ** valy us vs
+  ; e_starValid : forall tus tvs x y val,
+                    exprD' tus tvs SL (SSL.(e_star) x y) = Some val ->
+                    exists valx valy,
+                      exprD' tus tvs SL x = Some valx /\
+                      exprD' tus tvs SL y = Some valy /\
+                      forall us vs, val us vs -|- valx us vs ** valy us vs
+  ; e_andOk : forall tus tvs x y valx valy,
+                exprD' tus tvs SL x = Some valx ->
+                exprD' tus tvs SL y = Some valy ->
+                exists val,
+                  exprD' tus tvs SL (SSL.(e_and) x y) = Some val /\
+                  forall us vs, val us vs -|- valx us vs //\\ valy us vs
+  ; e_andValid : forall tus tvs x y val,
+                   exprD' tus tvs SL (SSL.(e_and) x y) = Some val ->
+                   exists valx valy,
+                     exprD' tus tvs SL x = Some valx /\
+                     exprD' tus tvs SL y = Some valy /\
+                     forall us vs, val us vs -|- valx us vs //\\ valy us vs
+  }.
+
+  Variable SSLO : SynSepLogOk.
+
+  (*
+    Local Instance PureOp_it : @PureOp _  := slsok.(_PureOp).
+    Local Instance Pure_it : @Pure _ _ _ slsok.(_PureOp) := _Pure slsok.
+    Hypothesis pure_ltrue : Pure.pure ltrue.
+    Hypothesis pure_land : forall p q, Pure.pure p -> Pure.pure q -> Pure.pure (land p q).
+   *)
+
+  Ltac forward_ex_and :=
+    repeat match goal with
+             | H : exists x, _ |- _ => destruct H
+             | H : _ /\ _ |- _ => destruct H
+           end.
+
+(*
+  (** Primed versions **)
+  Lemma exprD'_e_andOk_None1
+  : forall us tvs x y,
+      exprD' us tvs x SL = None ->
+      exprD' us tvs (SSL.(e_and) x y) SL = None.
+  Proof.
+    intros.
+    consider (exprD' us tvs (SSL.(e_and) x y) SL); auto; intros.
+    exfalso.
+    eapply e_andValid in H0; eauto. forward_ex_and. congruence.
+  Qed.
+
+  Lemma exprD'_e_andOk_None2
+  : forall us tvs x y,
+      exprD' us tvs y SL = None ->
+      exprD' us tvs (SSL.(e_and) x y) SL = None.
+  Proof.
+    intros.
+    consider (exprD' us tvs (SSL.(e_and) x y) SL); auto; intros.
+    exfalso.
+    eapply e_andValid in H0; eauto. forward_ex_and. congruence.
+  Qed.
+
+  Lemma exprD'_e_starOk_None1
+  : forall us tvs x y,
+      exprD' us tvs x SL = None ->
+      exprD' us tvs (SSL.(e_star) x y) SL = None.
+  Proof.
+    intros.
+    consider (exprD' us tvs (SSL.(e_star) x y) SL); auto; intros.
+    exfalso.
+    eapply e_starValid in H0; eauto. forward_ex_and. congruence.
+  Qed.
+
+  Lemma exprD'_e_starOk_None2
+  : forall us tvs x y,
+      exprD' us tvs y SL = None ->
+      exprD' us tvs (SSL.(e_star) x y) SL = None.
+  Proof.
+    intros.
+    consider (exprD' us tvs (SSL.(e_star) x y) SL); auto; intros.
+    exfalso.
+    eapply e_starValid in H0; eauto. forward_ex_and. congruence.
+  Qed.
+
+  Lemma exprD'_e_and_None
+  : forall us tvs a b,
+      exprD' us tvs (SSL.(e_and) a b) SL = None ->
+      exprD' us tvs a SL = None \/ exprD' us tvs b SL = None.
+  Proof.
+    intros.
+    consider (exprD' us tvs a SL); intros; auto.
+    consider (exprD' us tvs b SL); intros; auto.
+    exfalso.
+    destruct (@e_andOk SSLO _ _ _ _ _ _ H0 H1).
+    intuition; congruence.
+  Qed.
+
+  Lemma exprD'_e_star_None
+  : forall us tvs a b,
+      exprD' us tvs (SSL.(e_star) a b) SL = None ->
+      exprD' us tvs a SL = None \/ exprD' us tvs b SL = None.
+  Proof.
+    intros.
+    consider (exprD' us tvs a SL); intros; auto.
+    consider (exprD' us tvs b SL); intros; auto.
+    exfalso.
+    destruct (@e_starOk SSLO _ _ _ _ _ _ H0 H1).
+    intuition; congruence.
+  Qed.
+
+  (** Unprimed versions **)
+  Lemma exprD_e_andOk_None1
+  : forall us vs x y,
+      exprD us vs x SL = None ->
+      exprD us vs (SSL.(e_and) x y) SL = None.
+  Proof.
+    intros.
+    consider (exprD us vs (SSL.(e_and) x y) SL); auto; intros.
+    exfalso.
+    unfold exprD in *. destruct (split_env vs).
+    forward.
+    eapply e_andValid in H1; eauto. forward_ex_and. 
+    simpl in *. congruence.
+  Qed.
+
+  Lemma exprD_e_andOk_None2
+  : forall us vs x y,
+      exprD us vs y SL = None ->
+      exprD us vs (SSL.(e_and) x y) SL = None.
+  Proof.
+    intros.
+    consider (exprD us vs (SSL.(e_and) x y) SL); auto; intros.
+    exfalso.
+    unfold exprD in *. destruct (split_env vs).
+    forward.
+    eapply e_andValid in H1; eauto. forward_ex_and. simpl in *; congruence.
+  Qed.
+
+  Lemma exprD_e_starOk_None1
+  : forall us vs x y,
+      exprD us vs x SL = None ->
+      exprD us vs (SSL.(e_star) x y) SL = None.
+  Proof.
+    intros.
+    consider (exprD us vs (SSL.(e_star) x y) SL); auto; intros.
+    exfalso.
+    unfold exprD in *. destruct (split_env vs).
+    forward.
+    eapply e_starValid in H1; eauto. forward_ex_and. simpl in *; congruence.
+  Qed.
+
+  Lemma exprD_e_starOk_None2
+  : forall us vs x y,
+      exprD us vs y SL = None ->
+      exprD us vs (SSL.(e_star) x y) SL = None.
+  Proof.
+    intros.
+    consider (exprD us vs (SSL.(e_star) x y) SL); auto; intros.
+    exfalso.
+    unfold exprD in *. destruct (split_env vs).
+    forward.
+    eapply e_starValid in H1; eauto. forward_ex_and. simpl in *; congruence.
+  Qed.
+
+  Lemma exprD_e_and_None
+  : forall us vs a b,
+      exprD us vs (SSL.(e_and) a b) SL = None ->
+      exprD us vs a SL = None \/ exprD us vs b SL = None.
+  Proof.
+    intros.
+    consider (exprD us vs a SL); intros; auto.
+    consider (exprD us vs b SL); intros; auto.
+    exfalso.
+    unfold exprD in *. destruct (split_env vs).
+    forward.
+    destruct (@e_andOk SSLO _ _ _ _ _ _ H1 H2).
+    simpl in *; intuition; congruence.
+  Qed.
+
+  Lemma exprD_e_star_None
+  : forall us vs a b,
+      exprD us vs (SSL.(e_star) a b) SL = None ->
+      exprD us vs a SL = None \/ exprD us vs b SL = None.
+  Proof.
+    intros.
+    consider (exprD us vs a SL); intros; auto.
+    consider (exprD us vs b SL); intros; auto.
+    exfalso.
+    unfold exprD in *. destruct (split_env vs).
+    forward.
+    destruct (@e_starOk SSLO _ _ _ _ _ _ H1 H2).
+    simpl in *; intuition; congruence.
+  Qed.
+
+  Lemma exprD_e_empOk
+  : forall us vs,
+    exists val : typD ts nil SL,
+      exprD us vs SSL.(e_emp) SL = Some val /\
+      (val -|- empSP).
+  Proof.
+    unfold exprD; intros; destruct (split_env vs); destruct (split_env us).
+    destruct (SSLO.(e_empOk) x0 x) as [ ? [ ? ? ] ].
+    simpl in *. rewrite H. eauto.
+  Qed.
+
+  Lemma exprD_e_trueOk
+  : forall us vs,
+    exists val,
+      exprD us vs SSL.(e_true) SL = Some val /\
+      (val -|- ltrue).
+  Proof.
+    unfold exprD; intros; destruct (split_env vs); destruct (split_env us).
+    destruct (SSLO.(e_trueOk) x0 x) as [ ? [ ? ? ] ].
+    simpl in *; rewrite H. eauto.
+  Qed.
+
+  Lemma exprD_e_starOk
+  : forall us vs x y valx valy,
+      exprD us vs x SL = Some valx ->
+      exprD us vs y SL = Some valy ->
+      exists val,
+        exprD us vs (SSL.(e_star) x y) SL = Some val /\
+        (val -|- valx ** valy).
+  Proof.
+    unfold exprD; intros; destruct (split_env vs); destruct (split_env us).
+    forward.
+    destruct (@e_starOk SSLO x1 x0 x y _ _ H H0) as [ ? [ ? ? ] ].
+    simpl in *; rewrite H3. inv_all; subst. eauto.
+  Qed.
+
+  Lemma exprD_e_starValid
+  : forall us vs x y val,
+      exprD us vs (SSL.(e_star) x y) SL = Some val ->
+      exists valx valy,
+        exprD us vs x SL = Some valx /\
+        exprD us vs y SL = Some valy /\
+        (val -|- valx ** valy).
+  Proof.
+    unfold exprD; intros; destruct (split_env vs); destruct (split_env us).
+    forward.
+    edestruct (@e_starValid SSLO x1 x0 x) as [ ? [ ? [ ? [ ? ? ] ] ] ]; eauto.
+    simpl in *; Cases.rewrite_all_goal.
+    inv_all; subst. eauto.
+  Qed.
+
+  Lemma exprD_e_andOk
+  : forall us vs x y valx valy,
+      exprD us vs x SL = Some valx ->
+      exprD us vs y SL = Some valy ->
+      exists val,
+        exprD us vs (SSL.(e_and) x y) SL = Some val /\
+        (val -|- valx //\\ valy).
+  Proof.
+    unfold exprD; intros; destruct (split_env vs); destruct (split_env us).
+    simpl in *; forward.
+    destruct (@e_andOk SSLO x1 x0 x y _ _ H H0) as [ ? [ ? ? ] ].
+    rewrite H3. inv_all; subst. eauto.
+  Qed.
+
+  Lemma exprD_e_andValid
+  : forall us vs x y val,
+      exprD us vs (SSL.(e_and) x y) SL = Some val ->
+      exists valx valy,
+        exprD us vs x SL = Some valx /\
+        exprD us vs y SL = Some valy /\
+        (val -|- valx //\\ valy).
+  Proof.
+    unfold exprD; intros; destruct (split_env vs); destruct (split_env us).
+    simpl in *; forward.
+    edestruct (@e_andValid SSLO x1 x0 x) as [ ? [ ? [ ? [ ? ? ] ] ] ]; eauto.
+    Cases.rewrite_all_goal.
+    inv_all; subst. eauto.
+  Qed.
+
+  Ltac go_crazy :=
+    match goal with
+      | H : exprD' _ _ _ _ = _ , H' : _ |- _ =>
+        rewrite H in H'
+      | H : exprD' _ _ _ _ = _ |- _ =>
+        rewrite H
+      | H : exprD' _ _ ?C _ = _
+            , H' : exprD' _ _ ?D _ = _
+        |- context [ exprD' ?A ?B (SSL.(e_and) ?C ?D) ?T ] =>
+        destruct (@e_andOk SSLO _ _ _ _ _ _ H H') as [ ? [ ? ? ] ]
+      | H : exprD' _ _ ?C _ = _
+            , H' : exprD' _ _ ?D _ = _
+        |- context [ exprD' ?A ?B (SSL.(e_star) ?C ?D) ?T ] =>
+        destruct (@e_starOk SSLO _ _ _ _ _ _ H H') as [ ? [ ? ? ] ]
+      | H : exprD' _ _ (SSL.(e_and) _ _) _ = _ |- _ =>
+        eapply SSLO.(e_andValid) in H ; destruct H as [ ? [ ? [ ? [ ? ? ] ] ] ]
+      | H : exprD' _ _ (SSL.(e_star) _ _) _ = _ |- _ =>
+        eapply SSLO.(e_starValid) in H ; destruct H as [ ? [ ? [ ? [ ? ? ] ] ] ]
+      | H : exprD' _ _ ?C _ = _
+            , H' : exprD' _ _ ?D _ = _
+                   , H'' : context [ exprD' ?A ?B (SSL.(e_star) ?C ?D) ?T ]
+        |- _ =>
+        destruct (@e_starOk SSLO _ _ _ _ _ _ H H') as [ ? [ ? ? ] ]
+      | H : exprD' _ _ ?C _ = _
+            , H' : exprD' _ _ ?D _ = _
+                   , H'' : context [ exprD' ?A ?B (SSL.(e_and) ?C ?D) ?T ]
+        |- _ =>
+        destruct (@e_andOk SSLO _ _ _ _ _ _ H H') as [ ? [ ? ? ] ]
+      | H : exprD' _ _ _ _ = None |- _ =>
+        first [ erewrite (@exprD'_e_starOk_None1 _ _ _ _ H) in *
+              | erewrite (@exprD'_e_starOk_None2 _ _ _ _ H) in *
+              | erewrite (@exprD'_e_andOk_None1 _ _ _ _ H) in *
+              | erewrite (@exprD'_e_andOk_None2 _ _ _ _ H) in * ]
+
+      | H : exprD' _ _ _ _ = None |- _ =>
+        first [ congruence
+              | apply exprD'_e_star_None in H; destruct H; try congruence
+              | apply exprD'_e_and_None in H; destruct H; try congruence ]
+
+              (** **)
+      | H : exprD _ _ _ _ = _ , H' : _ |- _ =>
+        rewrite H in H'
+      | H : exprD _ _ _ _ = _ |- _ =>
+        rewrite H
+      | H : exprD _ _ ?C _ = _
+        , H' : exprD _ _ ?D _ = _
+        |- context [ exprD ?A ?B (SSL.(e_and) ?C ?D) ?T ] =>
+        destruct (@exprD_e_andOk _ _ _ _ _ _ H H') as [ ? [ ? ? ] ]
+      | H : exprD _ _ ?C _ = _
+        , H' : exprD _ _ ?D _ = _
+        |- context [ exprD ?A ?B (SSL.(e_star) ?C ?D) ?T ] =>
+        destruct (@exprD_e_starOk _ _ _ _ _ _ H H') as [ ? [ ? ? ] ]
+      | H : exprD _ _ (SSL.(e_and) _ _) _ = _ |- _ =>
+        eapply (@exprD_e_andValid) in H ; destruct H as [ ? [ ? [ ? [ ? ? ] ] ] ]
+      | H : exprD _ _ (SSL.(e_star) _ _) _ = _ |- _ =>
+        eapply (@exprD_e_starValid) in H ; destruct H as [ ? [ ? [ ? [ ? ? ] ] ] ]
+      | H : exprD _ _ ?C _ = _
+            , H' : exprD _ _ ?D _ = _
+                   , H'' : context [ exprD ?A ?B (SSL.(e_star) ?C ?D) ?T ]
+        |- _ =>
+        destruct (@e_starOk SSLO _ _ _ _ _ _ H H') as [ ? [ ? ? ] ]
+      | H : exprD _ _ ?C _ = _
+            , H' : exprD _ _ ?D _ = _
+                   , H'' : context [ exprD ?A ?B (SSL.(e_and) ?C ?D) ?T ]
+        |- _ =>
+        destruct (@e_andOk SSLO _ _ _ _ _ _ H H') as [ ? [ ? ? ] ]
+      | H : exprD _ _ _ _ = None |- _ =>
+        first [ erewrite (@exprD_e_starOk_None1 _ _ _ _ H) in *
+              | erewrite (@exprD_e_starOk_None2 _ _ _ _ H) in *
+              | erewrite (@exprD_e_andOk_None1 _ _ _ _ H) in *
+              | erewrite (@exprD_e_andOk_None2 _ _ _ _ H) in * ]
+
+      | H : exprD _ _ _ _ = None |- _ =>
+        first [ congruence
+              | apply exprD_e_star_None in H; destruct H; try congruence
+              | apply exprD_e_and_None in H; destruct H; try congruence ]
+    end.
+
+  Local Instance Reflexive_lentails : Reflexive lentails.
+  Proof.
+    destruct IL. destruct lentailsPre. auto.
+  Qed.
+
+  Lemma Sem_equiv_e_and_assoc
+  : forall us vs, forall a b c : expr sym,
+      Sem_equiv _ SL lequiv us vs
+                (SSL.(e_and) a (SSL.(e_and) b c))
+                (SSL.(e_and) (SSL.(e_and) a b) c).
+  Proof.
+    clear - IL SSL SSLO. intros.
+    red.
+    repeat match goal with
+             | |- context [ match ?X with _ => _ end ] =>
+               consider X; intros; auto; repeat go_crazy; auto
+           end.
+    inv_all. subst. Cases.rewrite_all_goal.
+    rewrite landA. reflexivity.
+  Qed.
+
+  Lemma Sem_equiv_e_star_assoc
+  : forall us vs, forall a b c : expr sym,
+      Sem_equiv _ SL lequiv us vs (SSL.(e_star) a (SSL.(e_star) b c)) (SSL.(e_star) (SSL.(e_star) a b) c).
+  Proof.
+    clear - IL SSL SSLO BIL. intros.
+    red.
+    repeat match goal with
+             | |- context [ match ?X with _ => _ end ] =>
+               consider X; intros; auto; repeat go_crazy; auto
+           end.
+    inv_all. subst. Cases.rewrite_all_goal.
+    rewrite sepSPA. reflexivity.
+  Qed.
+
+  Lemma Sem_equiv_Proper_e_and
+  : forall us vs,
+      Proper (Sem_equiv _ SL lequiv us vs ==>
+              Sem_equiv _ SL lequiv us vs ==>
+              Sem_equiv _ SL lequiv us vs) SSL.(e_and).
+  Proof.
+    unfold Sem_equiv. do 3 red.
+    intros; match goal with
+              | |- match ?X with _ => _ end =>
+                consider X; intros
+            end; repeat go_crazy; forward; repeat go_crazy.
+    inv_all; subst.
+    Cases.rewrite_all_goal. reflexivity.
+  Qed.
+
+  Lemma Sem_equiv_Proper_e_star
+  : forall us vs,
+      Proper (Sem_equiv _ SL lequiv us vs ==>
+              Sem_equiv _ SL lequiv us vs ==>
+              Sem_equiv _ SL lequiv us vs) SSL.(e_star).
+  Proof.
+    unfold Sem_equiv. do 3 red.
+    intros; match goal with
+              | |- match ?X with _ => _ end =>
+                consider X; intros
+            end; repeat go_crazy; forward; repeat go_crazy.
+    inv_all; subst.
+    Cases.rewrite_all_goal. reflexivity.
+  Qed.
+
+  Lemma ltrue_unitL : forall a, land ltrue a -|- a.
+  Proof.
+    clear - IL; intros.
+    split.
+    { eapply landL2. reflexivity. }
+    { eapply landR; try reflexivity. eapply ltrueR. }
+  Qed.
+
+  Lemma ltrue_unitR : forall a, land a ltrue -|- a.
+  Proof.
+    clear - IL; intros.
+    split.
+    { eapply landL1. reflexivity. }
+    { eapply landR; try reflexivity. eapply ltrueR. }
+  Qed.
+
+  Lemma empSPR : forall a, a ** empSP -|- a.
+  Proof.
+    clear - BIL IL; intros.
+    rewrite sepSPC. rewrite empSPL. reflexivity.
+  Qed.
+
+  Lemma Sem_equiv_e_true_e_and_unitLL
+  : forall us vs, forall a : expr sym,
+      Sem_equiv _ SL lequiv us vs (SSL.(e_and) SSL.(e_true) a) a.
+  Proof.
+    red; intros.
+    destruct (exprD_e_trueOk us vs) as [ ? [ ? ? ] ].
+    repeat match goal with
+             | |- context [ match ?X with _ => _ end ] =>
+               consider X; intros; auto; repeat go_crazy; auto
+           end.
+    inv_all; subst.
+    Cases.rewrite_all_goal.
+    rewrite ltrue_unitL. reflexivity.
+  Qed.
+
+  Lemma Sem_equiv_e_true_e_and_unitLR
+  : forall us vs, forall a : expr sym,
+      Sem_equiv _ SL lequiv us vs (SSL.(e_and) a SSL.(e_true)) a.
+  Proof.
+    red; intros.
+    destruct (exprD_e_trueOk us vs) as [ ? [ ? ? ] ].
+    repeat match goal with
+             | |- context [ match ?X with _ => _ end ] =>
+               consider X; intros; auto; repeat go_crazy; auto
+           end.
+    inv_all; subst.
+    Cases.rewrite_all_goal.
+    rewrite ltrue_unitR. reflexivity.
+  Qed.
+
+  Lemma Sem_equiv_e_true_e_and_unitRL
+  : forall us vs, forall a : expr sym,
+      Sem_equiv _ SL lequiv us vs a (SSL.(e_and) SSL.(e_true) a).
+  Proof.
+    red; intros.
+    destruct (exprD_e_trueOk us vs) as [ ? [ ? ? ] ].
+    repeat match goal with
+             | |- context [ match ?X with _ => _ end ] =>
+               consider X; intros; auto; repeat go_crazy; auto
+           end.
+    inv_all; subst.
+    Cases.rewrite_all_goal.
+    rewrite ltrue_unitL. reflexivity.
+  Qed.
+
+  Lemma Sem_equiv_e_true_e_and_unitRR
+  : forall us vs, forall a : expr sym,
+      Sem_equiv _ SL lequiv us vs a (SSL.(e_and) a SSL.(e_true)).
+  Proof.
+    red; intros.
+    destruct (exprD_e_trueOk us vs) as [ ? [ ? ? ] ].
+    repeat match goal with
+             | |- context [ match ?X with _ => _ end ] =>
+               consider X; intros; auto; repeat go_crazy; auto
+           end.
+    inv_all; subst.
+    Cases.rewrite_all_goal.
+    rewrite ltrue_unitR. reflexivity.
+  Qed.
+
+  Lemma Sem_equiv_e_emp_e_star_unitLL
+  : forall us vs, forall a : expr sym,
+      Sem_equiv _ SL lequiv us vs (SSL.(e_star) SSL.(e_emp) a) a.
+  Proof.
+    red; intros.
+    destruct (exprD_e_empOk us vs) as [ ? [ ? ? ] ].
+    repeat match goal with
+             | |- context [ match ?X with _ => _ end ] =>
+               consider X; intros; auto; repeat go_crazy; auto
+           end.
+    inv_all; subst.
+    Cases.rewrite_all_goal.
+    rewrite empSPL. reflexivity.
+  Qed.
+
+  Lemma Sem_equiv_e_emp_e_star_unitLR
+  : forall us vs, forall a : expr sym,
+      Sem_equiv _ SL lequiv us vs (SSL.(e_star) a SSL.(e_emp)) a.
+  Proof.
+    red; intros.
+    destruct (exprD_e_empOk us vs) as [ ? [ ? ? ] ].
+    repeat match goal with
+             | |- context [ match ?X with _ => _ end ] =>
+               consider X; intros; auto; repeat go_crazy; auto
+           end.
+    inv_all; subst.
+    Cases.rewrite_all_goal.
+    rewrite empSPR. reflexivity.
+  Qed.
+
+  Lemma Sem_equiv_e_emp_e_star_unitRL
+  : forall us vs, forall a : expr sym,
+      Sem_equiv _ SL lequiv us vs a (SSL.(e_star) SSL.(e_emp) a).
+  Proof.
+    red; intros.
+    destruct (exprD_e_empOk us vs) as [ ? [ ? ? ] ].
+    repeat match goal with
+             | |- context [ match ?X with _ => _ end ] =>
+               consider X; intros; auto; repeat go_crazy; auto
+           end.
+    inv_all; subst.
+    Cases.rewrite_all_goal.
+    rewrite empSPL. reflexivity.
+  Qed.
+
+  Lemma Sem_equiv_e_emp_e_star_unitRR
+  : forall us vs, forall a : expr sym,
+      Sem_equiv _ SL lequiv us vs a (SSL.(e_star) a SSL.(e_emp)).
+  Proof.
+    red; intros.
+    destruct (exprD_e_empOk us vs) as [ ? [ ? ? ] ].
+    repeat match goal with
+             | |- context [ match ?X with _ => _ end ] =>
+               consider X; intros; auto; repeat go_crazy; auto
+           end.
+    inv_all; subst.
+    Cases.rewrite_all_goal.
+    rewrite empSPR. reflexivity.
+  Qed.
+*)
+End syn_sep_log.
+
+(*
+(** Ltac's local to a section are not re-introduced **)
+Ltac go_crazy SSL SSLO :=
+  match goal with
+    | [ H : exprD' _ _ _ _ = _ , H' : _ |- _ ] =>
+      rewrite H in H'
+    | [ H : exprD' _ _ _ _ = _ |- _ ] =>
+      rewrite H
+    | [ H : exprD' _ _ ?C _ = _
+      , H' : exprD' _ _ ?D _ = _
+      |- context [ exprD' ?A ?B (SSL.(e_and) ?C ?D) ?T ] ] =>
+      destruct (@e_andOk _ _ _ _ _ _ _ SSLO _ _ _ _ _ _ H H') as [ ? [ ? ? ] ]
+    | [ H : exprD' _ _ ?C _ = _
+      , H' : exprD' _ _ ?D _ = _
+      |- context [ exprD' ?A ?B (SSL.(e_star) ?C ?D) ?T ] ] =>
+      destruct (@e_starOk _ _ _ _ _ _ _ SSLO _ _ _ _ _ _ H H') as [ ? [ ? ? ] ]
+    | [ H : exprD' _ _ (SSL.(e_and) _ _) _ = _ |- _ ] =>
+      eapply SSLO.(e_andValid) in H ; destruct H as [ ? [ ? [ ? [ ? ? ] ] ] ]
+    | [ H : exprD' _ _ (SSL.(e_star) _ _) _ = _ |- _ ] =>
+      eapply SSLO.(e_starValid) in H ; destruct H as [ ? [ ? [ ? [ ? ? ] ] ] ]
+    | [ H : exprD' _ _ ?C _ = _
+      , H' : exprD' _ _ ?D _ = _
+      , H'' : context [ exprD' ?A ?B (SSL.(e_star) ?C ?D) ?T ]
+      |- _ ] =>
+      destruct (@e_starOk _ _ _ _ _ _ _ SSLO _ _ _ _ _ _ H H') as [ ? [ ? ? ] ]
+    | [ H : exprD' _ _ ?C _ = _
+      , H' : exprD' _ _ ?D _ = _
+      , H'' : context [ exprD' ?A ?B (SSL.(e_and) ?C ?D) ?T ]
+      |- _ ] =>
+      destruct (@e_andOk _ _ _ _ _ _ _ SSLO _ _ _ _ _ _ H H') as [ ? [ ? ? ] ]
+    | [ H : exprD' _ _ _ _ = None |- _ ] =>
+      first [ erewrite (@exprD'_e_starOk_None1 _ _ _ _ _ _ _ SSLO _ _ _ _ H) in *
+            | erewrite (@exprD'_e_starOk_None2 _ _ _ _ _ _ _ SSLO _ _ _ _ H) in *
+            | erewrite (@exprD'_e_andOk_None1 _ _ _ _ _ _ _ SSLO _ _ _ _ H) in *
+            | erewrite (@exprD'_e_andOk_None2 _ _ _ _ _ _ _ SSLO _ _ _ _ H) in * ]
+    | [ H : exprD' _ _ _ _ = None |- _ ] =>
+      first [ congruence
+            | apply (@exprD'_e_star_None _ _ _ _ _ _ _ _ SSLO) in H; destruct H; try congruence
+            | apply (@exprD'_e_and_None _ _ _ _ _ _ _ _ SSLO) in H; destruct H; try congruence ]
+
+
+    | [ H : exprD _ _ _ _ = _ , H' : _ |- _ ] =>
+      rewrite H in H'
+    | [ H : exprD _ _ _ _ = _ |- _ ] =>
+      rewrite H
+    | [ H : exprD _ _ ?C _ = _
+      , H' : exprD _ _ ?D _ = _
+      |- context [ exprD ?A ?B (SSL.(e_and) ?C ?D) ?T ] ] =>
+      destruct (@exprD_e_andOk _ _ _ _ _ _ _ _ SSLO _ _ _ _ _ _ H H') as [ ? [ ? ? ] ]
+    | [ H : exprD _ _ ?C _ = _
+      , H' : exprD _ _ ?D _ = _
+      |- context [ exprD ?A ?B (SSL.(e_star) ?C ?D) ?T ] ] =>
+      destruct (@exprD_e_starOk _ _ _ _ _ _ _ _ SSLO _ _ _ _ _ _ H H') as [ ? [ ? ? ] ]
+    | [ H : exprD _ _ (SSL.(e_and) _ _) _ = _ |- _ ] =>
+      eapply (@exprD_e_andValid _ _ _ _ _ _ _ _ SSLO) in H ; destruct H as [ ? [ ? [ ? [ ? ? ] ] ] ]
+    | [ H : exprD _ _ (SSL.(e_star) _ _) _ = _ |- _ ] =>
+      eapply (@exprD_e_starValid _ _ _ _ _ _ _ _ SSLO) in H ; destruct H as [ ? [ ? [ ? [ ? ? ] ] ] ]
+    | [ H : exprD _ _ ?C _ = _
+      , H' : exprD _ _ ?D _ = _
+      , H'' : context [ exprD ?A ?B (SSL.(e_star) ?C ?D) ?T ]
+      |- _ ] =>
+      destruct (@exprD_e_starOk _ _ _ _ _ _ _ SSLO _ _ _ _ _ _ H H') as [ ? [ ? ? ] ]
+    | [ H : exprD _ _ ?C _ = _
+      , H' : exprD _ _ ?D _ = _
+      , H'' : context [ exprD ?A ?B (SSL.(e_and) ?C ?D) ?T ]
+      |- _ ] =>
+      destruct (@exprD_e_andOk _ _ _ _ _ _ _ SSLO _ _ _ _ _ _ H H') as [ ? [ ? ? ] ]
+
+    | [ H : exprD _ _ _ _ = None |- _ ] =>
+      first [ erewrite (@exprD_e_starOk_None1 _ _ _ _ _ _ _ SSLO _ _ _ _ H) in *
+            | erewrite (@exprD_e_starOk_None2 _ _ _ _ _ _ _ SSLO _ _ _ _ H) in *
+            | erewrite (@exprD_e_andOk_None1 _ _ _ _ _ _ _ SSLO _ _ _ _ H) in *
+            | erewrite (@exprD_e_andOk_None2 _ _ _ _ _ _ _ SSLO _ _ _ _ H) in * ]
+
+    | [ H : exprD _ _ _ _ = None |- _ ] =>
+      first [ congruence
+            | apply (@exprD_e_star_None _ _ _ _ _ _ _ _ SSLO) in H; destruct H; try congruence
+            | apply (@exprD_e_and_None _ _ _ _ _ _ _ _ SSLO) in H; destruct H; try congruence ]
+  end.
+*)
